update eclib

eclib/JWord.ec
@@ -8,23 +8,26 @@ abstract theory BitWord.
 
 op size : {int | 0 < size} as gt0_size.
 
-clone FinType as Alphabet with 
+clone FinType as Alphabet with
   type t    <- bool,
   op   enum <- [true; false],
   op   card <- 2.
 
-clone include MonoArray with 
+clone include MonoArray with
   type elem <- bool,
   op dfl <- false,
   op size <- size
   rename "of_list"  as "bits2w"
          "to_list"  as "w2bits"
          "^tP$"     as "wordP"
-         "sub"      as "bits"  
+         "sub"      as "bits"
   proof ge0_size by (apply ltzW; apply gt0_size).
 
 (* -------------------------------------------------------------------- *)
 abbrev modulus = 2 ^ size.
+
+abbrev max_uint = modulus - 1.
+lemma max_uintS: max_uint + 1 = modulus by done.
 
 lemma ge2_modulus : 2 <= modulus.
 proof.
@@ -45,15 +48,15 @@ hint exact : ge0_size gt0_size gt0_modulus ge2_modulus ge0_modulus max_size.
 (* --------------------------------------------------------------------- *)
 (* Conversions with int                                                  *)
 
-op of_int (x:int) : t = 
+op of_int (x:int) : t =
   bits2w (int2bs size (x %% modulus))
 axiomatized by of_intE.
 
-op to_uint (w:t) = 
+op to_uint (w:t) =
   bs2int (w2bits w)
 axiomatized by to_uintE.
 
-op smod (i:int) = 
+op smod (i:int) =
   if 2^(size - 1) <= i then i - modulus
   else i.
 
@@ -87,7 +90,7 @@ proof. by apply to_uintK. qed.
 (*hint simplify of_uintK@1. *)
 hint simplify to_uintK'@0.
 
-lemma of_sintK (x:int) : 
+lemma of_sintK (x:int) :
    to_sint (of_int x) = smod (x %% modulus).
 proof. by rewrite to_sintE of_uintK. qed.
 
@@ -124,7 +127,7 @@ proof. by rewrite Core.inj_eq // (Core.can_inj _ _  to_uintK). qed.
 (* -------------------------------------------------------------------- *)
 op int_bit x i = (x%%modulus) %/ 2 ^ i %% 2 <> 0.
 
-lemma of_intwE x i :  
+lemma of_intwE x i :
    (of_int x).[i] = (0 <= i < size /\ int_bit x i).
 proof.
   rewrite of_intE; case (0 <= i < size) => /= hi; last by rewrite get_out.
@@ -134,15 +137,15 @@ qed.
 lemma zerowE i: zero.[i] = false.
 proof. by rewrite of_intwE /int_bit. qed.
 hint simplify zerowE.
-  
-lemma of_int_powm1 p i : 
+
+lemma of_int_powm1 p i :
   (of_int (2^p - 1)).[i] = (0 <= i < size /\ i < p).
 proof.
   case: (0 <= i < size) => [[h0i his] | hi]; last by rewrite get_out.
   case (0 <= p) => hp; last by rewrite pow_le0 1:/# /= /#.
   have aux : forall p, 0 <= p <= size => (of_int (2 ^ p - 1)).[i] = (true /\ i < p).
   + move=> {p hp} p hp.
-    rewrite of_intwE 1:// /int_bit /= (modz_small (2 ^ p - 1)). 
+    rewrite of_intwE 1:// /int_bit /= (modz_small (2 ^ p - 1)).
     + smt (gt0_pow2 pow_Mle).
     case (i < p) => hip /=.
     + have -> : p = ((p - i - 1) + 1) + i by ring.
@@ -156,15 +159,15 @@ proof.
   by rewrite modzMDl -(modzMDl 1 (-1) modulus) /= of_int_mod aux 1:// his.
 qed.
 
-lemma get_to_uint w i : w.[i] = (0 <= i < size /\ to_uint w %/ 2 ^ i %% 2 <> 0). 
+lemma get_to_uint w i : w.[i] = (0 <= i < size /\ to_uint w %/ 2 ^ i %% 2 <> 0).
 proof.
   case : (0 <= i < size) => hi;last by rewrite get_out.
   rewrite -{1}(to_uintK w) of_intwE hi /int_bit (modz_small _ modulus) 2://.
-  by apply bound_abs; apply to_uint_cmp.  
+  by apply bound_abs; apply to_uint_cmp.
 qed.
 
-lemma b2i_get w i : 0 <= i => b2i w.[i] = to_uint w %/ 2 ^ i %% 2. 
-proof. 
+lemma b2i_get w i : 0 <= i => b2i w.[i] = to_uint w %/ 2 ^ i %% 2.
+proof.
   move=> hi;rewrite get_to_uint hi.
   case (i < size) => his //=; 1: smt (modz_cmp).
   rewrite divz_small //; apply bound_abs.
@@ -177,21 +180,25 @@ proof.
   elim /intind: j.
   + by rewrite mkseq0 bs2int_nil /=.
   move=> j hj hrec; rewrite mkseqS 1:// bs2int_rcons.
-  rewrite size_mkseq max_ler 1:// /= hrec.  
+  rewrite size_mkseq max_ler 1:// /= hrec.
   have {2}->:= modz_pow_split (i+j+1) (i+j) (to_uint w) 2 _; 1: smt().
   have hij1 : 2 ^ (i + j + 1) = 2^(j+1) * 2^i.
   + rewrite pow_add 1:/# 1://;congr;ring.
   have hij : 2 ^ (i + j) = 2^j * 2^i.
   + rewrite pow_add 1:/# 1://;congr;ring.
   have h2i0 : 2 ^ i <> 0 by smt (gt0_pow2).
-  rewrite -addzA {2}hij1 -mulzA divzMDl 1://. 
-  rewrite {2}hij -mulzA divzMDl 1://. 
-  rewrite modzMDl !modz_pow2_div; 1,2:smt(). 
+  rewrite -addzA {2}hij1 -mulzA divzMDl 1://.
+  rewrite {2}hij -mulzA divzMDl 1://.
+  rewrite modzMDl !modz_pow2_div; 1,2:smt().
   have -> : i + j + 1 - (i + j) = 1 by ring.
   have -> : i + j - i = j by ring.
   rewrite -(pow_add 2 j 1) 1,2:// pow2_1 (modz_small _ (2^j * 2)).
-  + by apply bound_abs; smt (modz_cmp gt0_pow2).
-  by rewrite addzC mulzC b2i_get 1:/#.  
+  + apply bound_abs; split.
+     smt (modz_cmp to_uint_cmp gt0_pow2).
+    move=> ?.
+    rewrite -hrec.
+    smt (modz_cmp to_uint_cmp gt0_pow2).
+  by rewrite addzC mulzC b2i_get 1:/#.
 qed.
 
 lemma bitsE w k len : bits w k len = mkseq (fun (i:int) => w.[k+i]) len.
@@ -231,9 +238,9 @@ lemma zerowiE i: zerow.[i] = false.
 proof. apply zerowE. qed.
 
 lemma onewE i: onew.[i] = (0 <= i < size).
-proof. 
-  rewrite oneE; case (0 <= i < size) => hi; 2:by rewrite get_out.  
-  by rewrite of_int_powm1 //= 1:/# hi. 
+proof.
+  rewrite oneE; case (0 <= i < size) => hi; 2:by rewrite get_out.
+  by rewrite of_int_powm1 //= 1:/# hi.
 qed.
 
 lemma xorwE w1 w2 i: (w1 +^ w2).[i] = w1.[i] ^^ w2.[i].
@@ -251,7 +258,7 @@ proof.
   by rewrite orE; case (0 <= i < size) => hi;[ rewrite map2iE | rewrite !get_out].
 qed.
 
-lemma invwE (w:t) i: 
+lemma invwE (w:t) i:
   (invw w).[i] = (0 <= i < size /\ !w.[i]).
 proof. by rewrite invE mapE initE;case (0 <= i < _). qed.
 
@@ -263,7 +270,7 @@ hint simplify (zerowE, zerowiE, onewE, xorwE, andwE, invwE, orwE).
 
 (* -------------------------------------------------------------------- *)
 lemma onew_neq0: onew <> zerow.
-proof. 
+proof.
   apply/negP=> /wordP/(_ 0) /=.
   by rewrite negb_imply neqF.
 qed.
@@ -290,7 +297,7 @@ lemma andwC: commutative andw.
 proof. by move=> w1 w2; apply/wordP=> i h; rewrite !bwordE andbC. qed.
 
 lemma andwDl: left_distributive andw (+^).
-proof. move=> w1 w2 w3; apply/wordP=> i h; rewrite !bwordE smt. qed.
+proof. move=> w1 w2 w3; apply/wordP=> i h; rewrite !bwordE /#. qed.
 
 lemma andwK: idempotent andw.
 proof. by move=> x; apply/wordP=> i h; rewrite !bwordE andbb. qed.
@@ -318,13 +325,13 @@ instance bring with t
 pred unitw (w:t) = w = onew.
 op iandw (w:t) = if w = onew then onew else w.
 
-clone Ring.ComRing as WRing with 
+clone Ring.ComRing as WRing with
    type t <- t,
    op zeror <- zero,
    op ( + ) <- (+^),
    op [ - ] <- oppw,
    op oner  <- onew,
-   op ( * ) <- andw, 
+   op ( * ) <- andw,
    op invr  <- iandw,
    pred unit <- unitw
 proof *.
@@ -335,13 +342,13 @@ realize addNr.     proof. move=> ?;ring. qed.
 realize oner_neq0. proof. apply onew_neq0. qed.
 realize mulrA.     proof. apply andwA. qed.
 realize mulrC.     proof. apply andwC. qed.
-realize mul1r.     proof. move=> ?;ring. qed. 
-realize mulrDl.    proof. apply andwDl. qed. 
+realize mul1r.     proof. move=> ?;ring. qed.
+realize mulrDl.    proof. apply andwDl. qed.
 realize mulVr.     proof. move=> ?;rewrite /unitw /iandw => -> /=;ring. qed.
 realize unitout.   proof. by move=> x;rewrite /unitw /iandw => ->. qed.
 
-realize unitP. 
-proof. 
+realize unitP.
+proof.
 move=> x y; rewrite /unitw !wordP => + i Hi -/(_ i Hi).
 by rewrite andwE onewE Hi /#.
 qed.
@@ -371,10 +378,10 @@ lemma andw1_s w : andw w onew = w.
 proof. by apply WRing.mulr1. qed.
 
 lemma orw0 w : orw w zero = w.
-proof. by apply wordP => i hi. qed.  
+proof. by apply wordP => i hi. qed.
 
 lemma or0w w : orw zero w = w.
-proof. by apply wordP => i hi. qed.  
+proof. by apply wordP => i hi. qed.
 
 lemma orw1 w : orw w onew = onew.
 proof. by apply wordP => i hi /=; case (0 <= i < size). qed.
@@ -394,9 +401,52 @@ proof. move=> ->;apply andwK. qed.
 lemma orwK_s w1 w2 : w1 = w2 => orw w1 w2 = w1.
 proof. move=> ->;apply orwK. qed.
 
+lemma andw_invw w: andw w (invw w) = zerow.
+proof. by rewrite -xorw1; ring. qed.
+
+lemma nosmt orw_xorw w1 w2: orw w1 w2 = w1 +^ w2 +^ (andw w1 w2).
+proof.
+apply wordP => i Hi.
+rewrite orE !xorE andE !map2iE //.
+by case: w1.[i]; case: w2.[i].
+qed.
+
+lemma nosmt andw_orwDl: left_distributive andw orw.
+proof.
+by move=> x y z; rewrite !orw_xorw; ring.
+qed.
+
+lemma nosmt andw_orwDr: right_distributive andw orw.
+proof.
+by move=> x y z; rewrite !orw_xorw; ring.
+qed.
+
+lemma nosmt orw_andwDl: left_distributive orw andw.
+proof.
+by move=> x y z; rewrite !orw_xorw; ring.
+qed.
+
+lemma nosmt orw_andwDr: right_distributive orw andw.
+proof.
+by move=> x y z; rewrite !orw_xorw; ring.
+qed.
+
+lemma orwC x y: orw x y = orw y x.
+proof. by rewrite orw_xorw andwC (xorwC x) -orw_xorw. qed.
+
+lemma xorw_invw w: w +^ (invw w) = onew.
+proof.
+apply wordP => i Hi.
+rewrite xorE !map2iE // onewE invwE !Hi /=.
+by case: w.[i].
+qed.
+
+lemma orw_invw w: orw w (invw w) = onew.
+proof. by rewrite orw_xorw andw_invw -xorwA xorw0_s xorw_invw. qed.
+
 hint simplify (xor0w, xorw0_s, xorw1, xor1w,
                and0w, andw0, and1w, andw1_s,
-               or0w, orw0, orw1, or1w, 
+               or0w, orw0, orw1, or1w,
                xorwK_s, andwK_s, orwK_s).
 
 (* --------------------------------------------------------------------- *)
@@ -497,19 +547,19 @@ qed.
 lemma to_uintM (x y : t) : to_uint (x * y) = (to_uint x * to_uint y) %% modulus.
 proof. by rewrite mulE /ulift2 !of_uintK. qed.
 
-lemma to_uintD_small (x y : t) : to_uint x + to_uint y < modulus => 
+lemma to_uintD_small (x y : t) : to_uint x + to_uint y < modulus =>
   to_uint (x + y) = to_uint x + to_uint y.
-proof. 
-  move=> h;rewrite to_uintD modz_small 2://; smt (to_uint_cmp). 
+proof.
+  move=> h;rewrite to_uintD modz_small 2://; smt (to_uint_cmp).
 qed.
 
-lemma to_uintM_small (x y : t) : to_uint x * to_uint y < modulus => 
+lemma to_uintM_small (x y : t) : to_uint x * to_uint y < modulus =>
   to_uint (x * y) = (to_uint x * to_uint y).
-proof. 
-  move=> h;rewrite to_uintM modz_small 2://; smt (to_uint_cmp). 
+proof.
+  move=> h;rewrite to_uintM modz_small 2://; smt (to_uint_cmp).
 qed.
 
-clone export Ring.ComRing as WRingA with 
+clone export Ring.ComRing as WRingA with
    type t <- t,
    op zeror <- of_int 0,
    op ( + ) <- BitWord.( + ),
@@ -520,7 +570,7 @@ clone export Ring.ComRing as WRingA with
    pred unit  <- BitWord.unit proof *.
 
 realize addrA.
-proof. 
+proof.
   move=> x y z; rewrite addE /ulift2 !to_uintD -of_int_mod modzDmr.
   by rewrite -(of_int_mod (_ + to_uint z)) modzDml addrA.
 qed.
@@ -532,13 +582,13 @@ realize add0r.
 proof. by move=> x; rewrite addE /ulift2; cbv delta. qed.
 
 realize addNr.
-proof. 
+proof.
   move=> x; rewrite addE oppE /ulift2 /ulift1 of_uintK.
   by rewrite -of_int_mod modzDml addNz.
 qed.
 
 realize oner_neq0.
-proof. 
+proof.
   apply /negP => heq.
   have := of_uintK 1; rewrite heq of_uintK mod0z.
   rewrite modz_small //;smt (ge2_modulus).
@@ -556,9 +606,9 @@ realize mul1r.
 proof. by move=> x; rewrite mulE /ulift2 to_uint1. qed.
 
 realize mulrDl.
-proof. 
+proof.
   move=> x y z; rewrite !addE !mulE /ulift2.
-  rewrite !of_uintK -of_int_mod modzMml eq_sym.  
+  rewrite !of_uintK -of_int_mod modzMml eq_sym.
   by rewrite -of_int_mod modzDml modzDmr mulrDl.
 qed.
 
@@ -574,7 +624,7 @@ proof. by move=> x /negb_exists /=; apply choiceb_dfl. qed.
 abbrev (^) = WRingA.exp.
 
 lemma ofintS (n : int) : 0 <= n => of_int (n + 1) = of_int 1 + of_int n.
-proof. by rewrite of_intD addrC. qed. 
+proof. by rewrite of_intD addrC. qed.
 
 lemma to_uintB (x y: t) : y \ule x => to_uint (x - y) = to_uint x - to_uint y.
 proof.
@@ -643,7 +693,7 @@ instance ring with t
   op opp   = BitWord.([-])
   op mul   = BitWord.( * )
   op expr  = WRingA.exp
-  op ofint = BitWord.of_int 
+  op ofint = BitWord.of_int
 
   proof oner_neq0 by apply oner_neq0
   proof addr0     by apply addr0
@@ -663,9 +713,106 @@ instance ring with t
 
 (* --------------------------------------------------------------------- *)
 (* Exact arithmetic operations                                           *)
+(*
 op subc : t -> t -> bool -> bool * t.
 op addc : t -> t -> bool -> bool * t.
 op mulu : t -> t -> t * t.
+*)
+
+op borrow_sub x y b = to_uint x < to_uint y + b2i b.
+
+op subc (x y:t) (b: bool): bool * t = (borrow_sub x y b, x-(y+of_int (b2i b)))
+ axiomatized by subcE.
+
+lemma subcP x y c:
+ let (c',z) = subc x y c
+ in to_uint z - modulus * b2i c' = to_uint x - (to_uint y + b2i c).
+proof.
+rewrite subcE /borrow_sub /=.
+case: (to_uint y + b2i c = modulus) => ?.
+ rewrite to_uintD.
+ have -> /=: to_uint (- (y + of_int (b2i c))) = 0.
+  rewrite to_uintN to_uintD of_uintK (modz_small (b2i c)).
+   by apply bound_abs; smt(ge2_modulus).
+  by rewrite H modzz /=.
+ rewrite H modz_small.
+  by apply bound_abs; apply to_uint_cmp.
+ have ->: to_uint x < modulus by smt(to_uint_cmp).
+ smt().
+case: (to_uint x < to_uint y + b2i c) => ?/=.
+ have E: to_uint y + b2i c = to_uint (y + of_int (b2i c)).
+  rewrite to_uintD_small.
+   rewrite !of_uintK modz_small; first by  apply bound_abs; smt(ge2_modulus).
+   by case: c => /=?; smt(to_uint_cmp).
+  by rewrite of_uintK modz_small //; apply bound_abs; smt(ge2_modulus).
+ rewrite E b2i1 /= eqr_sub.
+ have ->: x - (y + of_int (b2i c)) = -((y + of_int (b2i c)) - x) by ring.
+ rewrite to_uintN -modzDl modz_small.
+  have ?: 0 < to_uint (y + of_int (b2i c) - x) <= `|modulus|.
+   rewrite to_uintB; first by rewrite uleE -E; smt().
+   rewrite -E; smt(to_uint_cmp).
+  smt(to_uint_cmp).
+ rewrite to_uintB; first by rewrite uleE -E; smt().
+ smt(to_uint_cmp).
+rewrite b2i0 /= to_uintB.
+ rewrite uleE to_uintD_small.
+  by rewrite of_uintK modz_small; smt(to_uint_cmp ge2_modulus).
+ rewrite of_uintK modz_small; first smt(ge2_modulus).
+ smt(ge2_modulus to_uint_cmp).
+by rewrite to_uintD of_uintK !modz_small; smt(ge2_modulus to_uint_cmp).
+qed.
+
+abbrev subc_borrow x y c = (subc x y c).`1.
+
+op carry_add x y c = modulus <= to_uint x + to_uint y + b2i c.
+
+lemma carry_addC x y c: carry_add x y c = carry_add y x c.
+proof. by rewrite /carry_add (addzC (to_uint x)). qed.
+
+op addc (x y: t) (c: bool) : bool * t = (carry_add x y c, x+y+of_int (b2i c))
+ axiomatized by addcE.
+
+lemma addcP x y c:
+ let (c',z) = addc x y c
+ in to_uint z + modulus * b2i c' = to_uint x + to_uint y + b2i c.
+proof.
+rewrite addcE !addE /ulift2 /= !of_uintK /= modzDmr modzDml /carry_add.
+have /= ?: to_uint x + to_uint y + b2i c < 2*modulus.
+ by move: (to_uint_cmp x) (to_uint_cmp y); smt().
+case: (modulus <= to_uint x + to_uint y + b2i c) => /= ?.
+ have {1}->: to_uint x + to_uint y + b2i c = to_uint x + to_uint y + b2i c - modulus + modulus
+  by ring.
+ rewrite b2i1 modzDr modz_small.
+  by apply bound_abs; smt(to_uint_cmp bound_abs).
+ by ring.
+by rewrite modz_small; smt(to_uint_cmp bound_abs).
+qed.
+
+abbrev addc_carry x y c = (addc x y c).`1.
+
+op mulhi (x y: t) : t =
+ of_int ((to_uint x * to_uint y) %/ modulus).
+
+lemma mulhiP (x y: t):
+ to_uint (x*y) + modulus * to_uint (mulhi x y) = to_uint x * to_uint y.
+proof.
+have [??] := (to_uint_cmp x).
+have [??] := (to_uint_cmp y).
+rewrite to_uintM to_uint_small.
+ apply divz_cmp; first smt().
+ split; first smt().
+ by move=> _; apply ltr_pmul.
+by rewrite {3}(divz_eq (to_uint x * to_uint y) modulus) /#.
+qed.
+
+lemma mulhi0 (x y: t):
+ to_uint x* to_uint y < modulus => to_uint (mulhi x y) = 0.
+proof.
+move=> ?; rewrite /mulhi divz_small //; apply bound_abs.
+split=> //; smt (to_uint_cmp).
+qed.
+
+op mulu (x y: t): t * t = (mulhi x y, x*y) axiomatized by muluE.
 
 (* --------------------------------------------------------------------- *)
 (* Bitwize operations                                                    *)
@@ -695,14 +842,14 @@ proof.
   move=> hk [h0j hjs];rewrite /int_bit modz_pow2_div 1:/# modz_dvd.
   + by apply (dvdz_exp2l 2 1) => /#.
   case: (0 <= j - k < size) => [ [hjk1 hjk2] | hjk]  /=;last first.
-  + have hlt : (j < k) by smt().   
+  + have hlt : (j < k) by smt().
     have ->: k = (k-j-1) + 1 + j by ring.
     rewrite -pow_add 1:/# 1:// -mulzA mulzK; 1: smt (gt0_pow2).
     by rewrite -pow_add 1:/# //= -mulzA modzMl.
   rewrite (modz_pow2_div size) 1:/# modz_dvd.
   + by apply (dvdz_exp2l 2 1) => /#.
   have {1}-> : j = (j - k) + k by ring.
-  by rewrite -pow_add 1,2:// divzMpr 1:gt0_pow2. 
+  by rewrite -pow_add 1,2:// divzMpr 1:gt0_pow2.
 qed.
 
 lemma int_bitDP i j k : 0 <= i < modulus => 0 <= k => 0 <= j < size =>
@@ -723,10 +870,10 @@ proof.
     + apply bound_abs;apply modz_cmp;apply gt0_pow2.
     rewrite /= divzMDl. smt (gt0_pow2).
     rewrite (divz_small (im %/ 2 ^ k) (2 ^ j)) 2://.
-    apply bound_abs; apply divz_cmp; 1:by apply gt0_pow2. 
+    apply bound_abs; apply divz_cmp; 1:by apply gt0_pow2.
     by rewrite pow_add 1,2://;apply modz_cmp;apply gt0_pow2.
   rewrite /= (divz_small (i %/ 2 ^ k) (2 ^ j)) 2://.
-  apply bound_abs;apply divz_cmp; 1: by apply gt0_pow2.  
+  apply bound_abs;apply divz_cmp; 1: by apply gt0_pow2.
   rewrite pow_add 1,2://;smt (pow_Mle).
 qed.
 
@@ -742,23 +889,23 @@ proof.
   by apply modz_cmp.
 qed.
 
-lemma to_uint_shl (w:t) i : 
+lemma to_uint_shl (w:t) i :
   0 <= i => to_uint (w `<<<` i) = (to_uint w * 2^ i) %% modulus.
 proof.
   by move=> hi; rewrite -{1}(to_uintK w) shlMP 1:// of_uintK.
 qed.
 
-lemma to_uint_shr (w:t) i : 
+lemma to_uint_shr (w:t) i :
   0 <= i => to_uint (w `>>>` i) = to_uint w %/ 2^ i.
 proof.
   move=> hi;rewrite -{1}(to_uintK w) shrDP 1:// of_uintK.
-  rewrite (modz_small (to_uint w)).  
+  rewrite (modz_small (to_uint w)).
   + by apply bound_abs; apply to_uint_cmp.
   rewrite modz_small 2://.
   apply bound_abs; apply divz_cmp; [apply gt0_pow2 | ].
   smt (to_uint_cmp gt0_pow2).
 qed.
-    
+
 lemma shrw_shlw w i : w `>>>` i = w `<<<` (-i).
 proof. by apply wordP => k hk /=. qed.
 
@@ -788,19 +935,19 @@ proof.
 qed.
 hint simplify (shlw_add, shlw_out).
 
-lemma shrw_map2 f w1 w2 i : f false false = false => 
+lemma shrw_map2 f w1 w2 i : f false false = false =>
    (map2 f) (w1 `>>>` i) (w2 `>>>` i) = (map2 f w1 w2) `>>>` i.
 proof.
-  move=> hf;apply wordP => k hk. 
+  move=> hf;apply wordP => k hk.
   rewrite map2iE // !shrwE hk.
   case: (0 <= k + i < size) => hki; 1: by rewrite map2iE.
   by rewrite !get_out.
 qed.
 
-lemma shlw_map2 f w1 w2 i : f false false = false => 
+lemma shlw_map2 f w1 w2 i : f false false = false =>
    (map2 f) (w1 `<<<` i) (w2 `<<<` i) = (map2 f w1 w2) `<<<` i.
 proof.
-  move=> hf;apply wordP => k hk. 
+  move=> hf;apply wordP => k hk.
   rewrite map2iE // !shlwE hk.
   case: (0 <= k - i < size) => hki; 1: by rewrite map2iE.
   by rewrite !get_out.
@@ -826,29 +973,29 @@ proof. by rewrite orE shlw_map2. qed.
 
 hint simplify (shrw_and, shrw_xor, shrw_or, shlw_and, shlw_xor, shlw_or).
 
-op ror (x : t) (i : int) = 
+op ror (x : t) (i : int) =
   init (fun j => x.[(j + i) %% size])
 axiomatized by rorE.
 
-op rol (x : t) (i : int) = 
+op rol (x : t) (i : int) =
   init (fun j => x.[(j - i) %% size])
 axiomatized by rolE.
 
-lemma rorwE w k i : 
+lemma rorwE w k i :
   (ror w k).[i] = if (0 <= i < size) then w.[(i+k) %% size] else false.
 proof. by rewrite rorE initE. qed.
 
-lemma rolwE w k i : 
+lemma rolwE w k i :
   (rol w k).[i] = if (0 <= i < size) then w.[(i-k) %% size] else false.
 proof. by rewrite rolE initE. qed.
 
 hint simplify (rorwE, rolwE).
 
-lemma rol_xor w i : 0 <= i < size => 
+lemma rol_xor w i : 0 <= i < size =>
   rol w i = (w `<<<` i) `^` (w `>>>` (size - i)).
 proof.
   move=> hi; apply wordP => k hk /=.
-  rewrite hk /=. 
+  rewrite hk /=.
   case (0 <= k - i < size) => hki.
   + rewrite modz_small; 1: by apply bound_abs.
     by rewrite (get_out _ (k + (size - i))) 1:/#.
@@ -856,20 +1003,20 @@ proof.
   by congr;ring.
 qed.
 
-lemma rol_xor_simplify w1 w2 i si: 
-   w1 = w2 => si = size - i => 0 <= i < size => 
+lemma rol_xor_simplify w1 w2 i si:
+   w1 = w2 => si = size - i => 0 <= i < size =>
    (w1 `<<<` i) `^` (w2 `>>>` si) = rol w1 i.
 proof. by move=> 2!-> hi;rewrite rol_xor. qed.
 
 (* --------------------------------------------------------------------- *)
 (* Like between bitwize operations and arithmetic operations             *)
 
-lemma and_mod k w : 
-  0 <= k => 
+lemma and_mod k w :
+  0 <= k =>
     w `&` of_int (2^k - 1) = of_int (to_uint w %% 2^k).
 proof.
   move=> hk;apply wordP => i hi /=.
-  rewrite of_int_powm1 of_intwE hi /= /int_bit.  
+  rewrite of_int_powm1 of_intwE hi /= /int_bit.
   rewrite (modz_small _ modulus).
   + apply bound_abs; smt (le_modz modz_cmp to_uint_cmp gt0_pow2).
   case (i < k) => hik /=.
@@ -879,12 +1026,356 @@ proof.
   rewrite divz_small 2://; smt (gt0_pow2 modz_cmp pow_Mle).
 qed.
 
-lemma to_uint_and_mod k w : 
-  0 <= k => 
+lemma to_uint_and_mod k w :
+  0 <= k =>
     to_uint (w `&` of_int (2^k - 1)) = to_uint w %% 2^k.
 proof.
-  move=> hk ; rewrite and_mod 1:// of_uintK modz_small //. 
+  move=> hk ; rewrite and_mod 1:// of_uintK modz_small //.
   apply bound_abs; smt (le_modz to_uint_cmp gt0_pow2 modz_cmp).
+qed.
+
+lemma nosmt to_uintNE w:
+ to_uint (-w) = (modulus - to_uint w) %% modulus.
+proof.
+rewrite to_uintN.
+by have /= ->:= (modzMDl 1).
+qed.
+
+lemma nosmt of_intNE (n:int):
+  of_int (-n) = of_int (modulus - n).
+proof.
+rewrite of_intN.
+apply word_modeqP; congr.
+rewrite to_uintN !of_uintK modzNm.
+by have /= ->:= (modzMDl 1).
+qed.
+
+lemma of_int_modulus: of_int modulus = BitWord.zero.
+proof. rewrite !of_intE modzz modz_small; smt(gt0_modulus). qed.
+
+lemma to_uint_onew: to_uint onew = max_uint.
+proof. by rewrite oneE of_uintK modz_small //; smt(ge2_modulus). qed.
+
+lemma onewS: onew + BitWord.one = BitWord.zero.
+proof.
+apply word_modeqP; congr.
+by rewrite to_uintD to_uint0 to_uint_onew to_uint1 max_uintS modzz.
+qed.
+
+lemma nosmt to_uintD_disjoint w1 w2:
+ w1 `&` w2 = BitWord.zero =>
+ to_uint (w1 + w2) = to_uint w1 + to_uint w2.
+proof.
+move=> H; have ?: to_uint (w1 `&` w2) = 0 by smt(to_uint0).
+rewrite to_uintD_small //.
+move: H0; rewrite !to_uintE.
+rewrite andE => ?.
+apply bs2int_add_disjoint.
+  by rewrite !size_map !size_iota.
+ by rewrite !size_map !size_iota max_ler.
+rewrite -H0; congr.
+rewrite map2_w2bits bits2wK //.
+by rewrite size_map2 min_ler !size_w2bits.
+qed.
+
+lemma nosmt orw_disjoint w1 w2:
+ w1 `&` w2 = BitWord.zero => w1 `|` w2 = w1 + w2.
+proof.
+move=> H; have ?: to_uint (w1 `&` w2) = 0 by smt(to_uint0).
+apply word_modeqP; congr.
+rewrite to_uintD_disjoint //.
+move: H0; rewrite !to_uintE andE => ?.
+rewrite orE.
+rewrite -bs2int_or_add ?size_mkseq //.
+ rewrite -H0.
+ rewrite map2_w2bits bits2wK.
+  by rewrite size_map2 min_ler !size_w2bits.
+ done.
+rewrite map2_w2bits bits2wK.
+ by rewrite size_map2 min_ler !size_w2bits.
+done.
+qed.
+
+lemma nosmt to_uint_orw_disjoint w1 w2:
+ w1 `&` w2 = zero =>
+ to_uint (w1 `|` w2) = to_uint w1 + to_uint w2.
+proof. by move=> *; rewrite orw_disjoint // to_uintD_disjoint. qed.
+
+lemma nosmt ule_andN0 (x y: t):
+ x `&` invw y = BitWord.zero =>
+ x \ule y.
+proof.
+rewrite andwC => ?; have: to_uint (invw y `&` x) = 0 by smt(to_uint0).
+rewrite !to_uintE andE invE => ?.
+have ->: x \ule y = (0 <= (to_uint y - to_uint x)) by rewrite uleE /#.
+rewrite !to_uintE; apply bs2int_sub_common.
+ by rewrite !size_map !size_iota.
+rewrite -H0; congr.
+rewrite map2_w2bits bits2wK.
+ by rewrite size_map2 min_ler !size_w2bits.
+congr; rewrite /w2bits /mkseq -!map_comp /(\o) //=.
+apply eq_in_map => ?.
+rewrite mem_iota /=; move => [??].
+by rewrite mapiE /#.
+qed.
+
+lemma nosmt ule_andw x y:
+ x `&` y \ule x.
+proof.
+rewrite andwC; apply ule_andN0.
+by rewrite -andwA andw_invw andw0.
+qed.
+
+lemma nosmt to_uint_ule_andw (x y: t):
+ to_uint (x `&` y) <= to_uint x.
+proof. have := ule_andw x y; by rewrite uleE. qed.
+
+lemma nosmt ule_orw x y:
+ x \ule x `|` y.
+proof.
+have {1}->: x = (x`|`y) `&` (x`|`invw y).
+ rewrite -{1}orw0.
+ have :=(andw_invw y); rewrite /zerow => <-.
+ by rewrite orw_andwDr.
+by apply ule_andw.
+qed.
+
+lemma nosmt subw_xorw w1 w2:
+ invw w1 `&` w2 = BitWord.zero => w1 - w2 = w1 `^` w2.
+proof.
+move=> H; have ?: to_uint (invw w1 `&` w2) = 0 by smt(to_uint0).
+apply word_modeqP; congr.
+rewrite to_uintB.
+ by apply ule_andN0; rewrite andwC.
+move: H0; rewrite !to_uintE andE invE => ?.
+rewrite xorE.
+rewrite -bs2int_xor_sub ?size_mkseq //.
+ rewrite -H0.
+ rewrite map2_w2bits bits2wK.
+  by rewrite size_map2 min_ler !size_w2bits.
+ congr; congr.
+ rewrite /w2bits /mkseq -!map_comp /(\o) //=.
+ apply eq_in_map => x.
+ rewrite mem_iota /= => /> *.
+ by rewrite mapiE /#.
+rewrite map2_w2bits bits2wK.
+ by rewrite size_map2 min_ler !size_w2bits.
+done.
+qed.
+
+lemma nosmt orw_xpnd w1 w2: w1 `|` w2 = w1 - w1 `&` w2 + w2.
+proof.
+rewrite subw_xorw.
+ by rewrite andwA (andwC (invw w1)) andw_invw and0w.
+rewrite -orw_disjoint.
+ by rewrite andwDl -andwA andwK xorwK.
+rewrite !orw_xorw.
+have ->: w1 `^` (w1 `&` w2) `&` w2 = zerow.
+ by rewrite andwDl -andwA andwK xorwK.
+by rewrite -!xorwA xorw0 (xorwC w2).
+qed.
+
+lemma ones_compl w: w + invw w = onew.
+proof.
+have:= orw_invw w.
+rewrite orw_xpnd andw_invw => <-.
+by ring.
+qed.
+
+lemma nosmt twos_compl (x: t):  -x = invw x + BitWord.one.
+proof.
+apply (addrI x); rewrite addrA ones_compl onewS.
+by ring.
+qed.
+
+lemma minus_one: -one = onew.
+proof.
+rewrite twos_compl -orw_disjoint.
+ by rewrite andwC andw_invw.
+by rewrite orwC orw_invw.
+qed.
+
+lemma nosmt to_uint_invw w: to_uint (invw w) = max_uint - to_uint w.
+proof.
+rewrite -to_uint_onew -to_uintB.
+ rewrite uleE to_uint_onew.
+ smt(to_uint_cmp).
+by congr; rewrite -(ones_compl w); ring.
+qed.
+
+abbrev masklsb k = of_int (2^k - 1).
+
+lemma masklsbNeg k:
+ k <= 0 => masklsb k = zerow.
+proof. by move=> ?; rewrite powNeg //. qed.
+
+lemma masklsbE k i:
+ (masklsb k).[i] = 0 <= i < min k size.
+proof.
+case: (0 <= k) => ?; last by rewrite masklsbNeg /=; smt().
+case: (0 <= i < size) => Hi; last by rewrite get_out /#.
+rewrite of_intE.
+case: (size <= k) => ?.
+ rewrite powm1_mod // get_bits2w //.
+ have /= <-:= (bs2int_nseq true).
+ have:= bs2intK (nseq size true); rewrite size_nseq max_ler 1:/# => ->.
+ by rewrite nth_nseq // min_ler // Hi.
+rewrite modz_small; first by smt(gt0_pow2 pow_Mle).
+rewrite get_bits2w //.
+have /= <-:= (bs2int_nseq true).
+rewrite (bs2int_pad size).
+pose L:= _++_.
+have:= bs2intK L; rewrite size_cat !size_nseq !max_ler 1,2:/#.
+have -> ->: k + (size-k) = size by smt().
+rewrite /L nth_cat size_nseq max_ler //=.
+by case: (i < k) => ?; rewrite nth_nseq /#.
+qed.
+
+hint simplify masklsbE.
+
+(* same as to_uint_and_mod
+lemma to_uint_andmask k w:
+ 0 <= k =>
+ to_uint (w `&` masklsb k) = to_uint w %% 2^k.
+proof. by move=> ?; rewrite to_uint_and_mod. qed.
+*)
+
+lemma nosmt shrl_andmaskN k w:
+ 0 <= k =>
+ w `>>>` k `<<<` k = w `&` invw (masklsb k).
+proof. by move=> Hk; apply wordP => i Hi /= /#. qed.
+
+lemma nosmt shlw_andmask k1 k2 w:
+ 0 <= k1 <= k2 < size =>
+ (w `<<<` k1) `&` masklsb k2 = (w `&` masklsb (k2-k1)) `<<<` k1.
+proof.
+move=> *; apply/wordP => i Hi /=; rewrite !Hi /= /min.
+smt(get_out).
+qed.
+
+lemma nosmt andmask_shrw k1 k2 w:
+ 0 <= k2 < k1 < size =>
+ (w `&` masklsb k1) `>>>` k2
+ = (w `>>>` k2) `&` masklsb (k1-k2).
+proof.
+move=> *; apply/wordP => i Hi /=; rewrite !Hi /min /=.
+smt(get_out).
+qed.
+
+lemma nosmt andmask_shlw k1 k2 w:
+ 0 <= k1 < size =>
+ (w `&` masklsb k1) `<<<` k2
+ = (w `<<<` k2) `&` masklsb (k1+k2).
+proof.
+move=> *; apply/wordP => i Hi /=; rewrite Hi /= /min.
+smt(get_out).
+qed.
+
+lemma nosmt shrw_shlw_disjoint k1 k2 w1 w2:
+ 0 <= k1 < size <= k1+k2 =>
+ (w1 `>>>` k1) `&` (w2 `<<<` k2) = zero.
+proof.
+move=> *; apply/wordP => i Hi /=; rewrite Hi /= /min.
+smt(get_out).
+qed.
+
+lemma nosmt andmaskK k w:
+ size <= k =>  w `&` masklsb k = w.
+proof. by move=> *; apply/wordP => i Hi /= /#. qed.
+
+lemma nosmt shrw_andmaskK k1 k2 w:
+ 0 <= k1 < size <= (k1+k2)%Int =>
+ (w `>>>` k1) `&` masklsb k2 = (w `>>>` k1).
+proof.
+move=> *; apply/wordP => i Hi /=; rewrite !Hi /= /min.
+smt(get_out).
+qed.
+
+lemma mask_and_mask k1 k2:
+ 0 <= k1 => 0 <= k2 =>
+ (masklsb k1 `&` masklsb k2) = masklsb (min k1 k2).
+proof. by move=> *; apply/wordP => i Hi /= /#. qed.
+
+lemma nosmt shrw_shlw_shlw k1 k2 x:
+ 0 <= k1 < k2 =>
+ x `>>>` k1 `<<<` k2 = (x `&` invw (masklsb k1)) `<<<` (k2-k1).
+proof. by move=> *; apply/wordP => i Hi /= /#. qed.
+
+lemma nosmt shrw_shlw_shrw k1 k2 x:
+ 0 <= k2 <= k1 < size =>
+ x `>>>` k1 `<<<` k2 = (x `&` invw (masklsb k1)) `>>>` (k1-k2).
+proof.
+move=> *; apply/wordP => i Hi /=; rewrite !Hi /= /min.
+smt(get_out).
+qed.
+
+lemma nosmt shlw_shrw_shlw k1 k2 x:
+ 0 <= k2 <= k1 < size =>
+ x `<<<` k1 `>>>` k2 = (x `&` masklsb (size-k1)) `<<<` (k1-k2).
+proof.
+move=> *; apply/wordP => i Hi /=; rewrite !Hi /= /min.
+smt(get_out).
+qed.
+
+lemma nosmt shlw_shrw_shrw k1 k2 x:
+ 0 <= k1 < k2 < size =>
+ x `<<<` k1 `>>>` k2 = (x `&` masklsb (size-k1)) `>>>` (k2-k1).
+proof. by move=> *; apply/wordP => i Hi /=; rewrite !Hi /= /#. qed.
+
+lemma nosmt splitwE k w:
+ 0 <= k =>
+ to_uint w = to_uint (w `&` masklsb k) + 2^k * to_uint (w `>>>` k).
+proof.
+move=> ?; rewrite to_uint_and_mod // to_uint_shr //.
+by rewrite {1}(divz_eq (to_uint w) (2^k)); ring.
+qed.
+
+op splitBits k w = (w `&` masklsb k, w `>>>` k).
+
+lemma nosmt splitBits_disjoint k w:
+ 0 <= k =>
+ (splitBits k w).`1 `&` ((splitBits k w).`2 `<<<` k) = BitWord.zero.
+proof.
+move => *; rewrite /splitBits /= shrl_andmaskN //.
+by rewrite andwA -(andwA w) (andwC _ w) andwA andwK -andwA andw_invw andw0.
+qed.
+
+lemma nosmt to_uint_splitBits k w:
+ 0 <= k =>
+ to_uint (splitBits k w).`1 + 2^k * to_uint (splitBits k w).`2 = to_uint w.
+proof. by move=> ?; rewrite eq_sym (splitwE k w). qed.
+
+op splitMask mask w = (w `&` mask, w `&` invw mask).
+
+abbrev splitAt k = splitMask (masklsb k).
+
+lemma splitMask_and0 mask w:
+ (splitMask mask w).`1 `&` (splitMask mask w).`2 = BitWord.zero.
+proof.
+rewrite /splitMask /=.
+by rewrite (andwC w) -andwA (andwA w) andwK (andwC w) andwA andw_invw and0w.
+qed.
+
+lemma nosmt splitMask_add mask w:
+ (splitMask mask w).`1 + (splitMask mask w).`2 = w.
+proof.
+rewrite -orw_disjoint; first by apply (splitMask_and0 mask w).
+by rewrite /splitMask /= !(andwC w) -andw_orwDl orw_invw and1w.
+qed.
+
+lemma nosmt splitAtP k w:
+ 0 <= k <= size =>
+ to_uint (splitAt k w).`1 = to_uint w %% 2^k
+ /\ to_uint (splitAt k w).`2 = 2^k * (to_uint w %/ 2^k).
+proof.
+move=> /> *.
+rewrite /splitMask /= -shrl_andmaskN //; split.
+ by rewrite to_uint_and_mod.
+rewrite to_uint_shl // to_uint_shr // modz_small //; last by smt(to_uint_cmp).
+apply bound_abs; split.
+ smt(divr_ge0 divz_ge0 gt0_pow2 to_uint_cmp).
+move=> *.
+by apply (ler_lt_trans (to_uint w)); smt(leq_trunc_div gt0_pow2 to_uint_cmp).
 qed.
 
 end BitWord.
@@ -895,7 +1386,7 @@ theory W8.
   proof gt0_size by done.
 
   op (`>>`) (w1 w2 : W8.t) = w1 `>>>` (to_uint w2 %% size).
-  op (`<<`) (w1 w2 : W8.t) = w1 `<<<` (to_uint w2 %% size). 
+  op (`<<`) (w1 w2 : W8.t) = w1 `<<<` (to_uint w2 %% size).
 
   lemma shr_div w1 w2 : to_uint (w1 `>>` w2) = to_uint w1 %/ 2^ (to_uint w2 %% size).
   proof.
@@ -905,7 +1396,7 @@ theory W8.
     by have:= to_uint_cmp w1; smt (gt0_pow2).
   qed.
 
-  lemma shr_div_le w1 i : 0 <= i < size => 
+  lemma shr_div_le w1 i : 0 <= i < size =>
        to_uint (w1 `>>` (of_int i)) = to_uint w1 %/ 2^i.
   proof.
     move=> hi;rewrite shr_div of_uintK.
@@ -913,13 +1404,13 @@ theory W8.
     by rewrite modz_small.
   qed.
 
-  lemma rol_xor_shft w i : 0 < i < size => 
+  lemma rol_xor_shft w i : 0 < i < size =>
     rol w i = (w `<<` of_int i) +^ (w `>>` of_int (size - i)).
   proof.
     move=> hi; rewrite /(`<<`) /(`>>`) !of_uintK /=.
     by rewrite !(modz_small _ 256) 1,2:/# !modz_small 1,2:/# rol_xor 1:/#.
   qed.
-end W8. export W8. 
+end W8. export W8.
 
 abstract theory WT.
   type t.
@@ -933,10 +1424,10 @@ abstract theory WT.
   op orw  : t -> t -> t.
   op (+^) : t -> t -> t.
   op invw : t -> t.
-  
+
   op (+) : t -> t -> t.
 
-  op (`>>`) : t -> W8.t -> t. 
+  op (`>>`) : t -> W8.t -> t.
   op (`<<`) : t -> W8.t -> t.
   op rol : t -> int -> t.
   op of_int : int -> t.
@@ -946,7 +1437,7 @@ abstract theory WT.
   op bits : t -> int -> int -> bool list.
 
   axiom initiE (f : int -> bool) (i : int) : 0 <= i < size => (init f).[i] = f i.
-  
+
   axiom andwE (w1 w2 : t) (i : int) : (andw w1 w2).[i] = (w1.[i] /\ w2.[i]).
   axiom orwE  (w1 w2 : t) (i : int) : (orw  w1 w2).[i] = (w1.[i] \/ w2.[i]).
   axiom xorwE (w1 w2 : t) (i : int) : (w1 +^ w2).[i] = (w1.[i] ^^ w2.[i]).
@@ -959,14 +1450,14 @@ abstract theory WT.
 
   op int_bit x i = (x%%2^size) %/ 2 ^ i %% 2 <> 0.
 
-  axiom of_intwE x i :  
+  axiom of_intwE x i :
    (of_int x).[i] = (0 <= i < size /\ int_bit x i).
 
-  axiom get_to_uint w i : w.[i] = (0 <= i < size /\ to_uint w %/ 2 ^ i %% 2 <> 0). 
+  axiom get_to_uint w i : w.[i] = (0 <= i < size /\ to_uint w %/ 2 ^ i %% 2 <> 0).
 
   axiom bitsE w k len : bits w k len = mkseq (fun (i:int) => w.[k+i]) len.
 
-  axiom bits_divmod w i j: 0 <= i => 0 <= j => 
+  axiom bits_divmod w i j: 0 <= i => 0 <= j =>
     bs2int (bits w i j) = ((to_uint w) %/ 2^i) %% 2^j.
 
   axiom to_uintRL (w:t) (x:int) : to_uint w = x %% 2^size => w = of_int x.
@@ -979,11 +1470,11 @@ abstract theory WT.
 
   axiom of_int_mod (x : int) : of_int (x %% 2^size) = of_int x.
 
-  axiom and_mod k w : 
-    0 <= k => 
+  axiom and_mod k w :
+    0 <= k =>
       andw w (of_int (2^k - 1)) = of_int (to_uint w %% 2^k).
 
-  axiom rol_xor_shft w i : 0 < i < size => 
+  axiom rol_xor_shft w i : 0 < i < size =>
     rol w i = (w `<<` W8.of_int i) +^ (w `>>` W8.of_int (size - i)).
 
 end WT.
@@ -991,7 +1482,7 @@ end WT.
 abstract theory W_WS.
 
   op sizeS : int.
-  op sizeB : int. 
+  op sizeB : int.
   op r : int.
   axiom gt0_r : 0 < r.
   axiom sizeBrS : sizeB = r * sizeS.
@@ -999,7 +1490,7 @@ abstract theory W_WS.
   clone import WT as WS with op size <- sizeS.
   clone import WT as WB with op size <- sizeB.
 
-  clone export MonoArray as Pack with 
+  clone export MonoArray as Pack with
     type elem <- WS.t,
     op dfl <- WS.of_int 0,
     op size <- r
@@ -1015,7 +1506,11 @@ abstract theory W_WS.
 
   lemma in_bound i j : 0 <= i < r => 0 <= j < sizeS => 0 <= i * sizeS + j < sizeB.
   proof.
-    move=> hi hj;rewrite sizeBrS;have : i * sizeS + j < (i+1) * sizeS; smt ().
+    move=> hi hj;rewrite sizeBrS;have : i * sizeS + j < (i+1) * sizeS by smt().
+    rewrite mulzDl /= => ?; split; first smt().
+    move => ?; apply (ltr_le_trans _ _ _ H).
+    have ->: i * sizeS + sizeS = (i+1)*sizeS by smt().
+    by apply ler_wpmul2r; smt().
   qed.
 
   (* ------------------------------------------------ *)
@@ -1024,7 +1519,7 @@ abstract theory W_WS.
   op zeroextu'B  (w:WS.t) = WB.of_int (WS.to_uint w).
   op truncateu'S (w:WB.t) = WS.of_int (WB.to_uint w).
 
-  hint exact : WS.gt0_size WB.gt0_size. 
+  hint exact : WS.gt0_size WB.gt0_size.
 
   lemma size_div : sizeS %| sizeB.
   proof. by rewrite dvdzP sizeBrS;exists r. qed.
@@ -1035,42 +1530,42 @@ abstract theory W_WS.
   op (\bits'S) (w:WB.t) i = WS.init (fun j => w.[ i * sizeS + j])
   axiomatized by bits'SE.
 
-  op unpack'S (w:WB.t) : pack_t = 
+  op unpack'S (w:WB.t) : pack_t =
     Pack.init (fun i => w \bits'S i).
 
   abbrev to_list (w:WB.t) : WS.t list = Pack.to_list (unpack'S w).
 
-  op pack'R_t (ws:pack_t) = 
+  op pack'R_t (ws:pack_t) =
     WB.init (fun i => ws.[i %/ sizeS].[i %% sizeS])
   axiomatized by pack'RE.
 
   abbrev pack'R (ws:WS.t list) = pack'R_t (Pack.of_list ws).
- 
-  lemma pack'RwE (ws:pack_t) i : 0 <= i < sizeB => 
+
+  lemma pack'RwE (ws:pack_t) i : 0 <= i < sizeB =>
     (pack'R_t ws).[i] = ws.[i %/ sizeS].[i %% sizeS].
   proof. by move=> hi;rewrite pack'RE initiE //. qed.
 
-  lemma get_unpack'S w i : 0 <= i < r => 
+  lemma get_unpack'S w i : 0 <= i < r =>
     (unpack'S w).[i] = w \bits'S i.
   proof. apply initiE. qed.
 
-  lemma bits'SiE w i j : 0 <= j < sizeS => 
+  lemma bits'SiE w i j : 0 <= j < sizeS =>
     (w \bits'S i).[j] = w.[i * sizeS + j].
   proof. by move=> hj; rewrite bits'SE initiE. qed.
-  
-  lemma get_bits'S (w:WB.t) i : 
-    0 <= i < sizeB => 
+
+  lemma get_bits'S (w:WB.t) i :
+    0 <= i < sizeB =>
     w.[i] = (w \bits'S (i%/ sizeS)).[i %% sizeS].
-  proof. 
+  proof.
     by move=> hi; rewrite bits'SE WS.initiE /= -?divz_eq; 1:by apply modz_cmp.
   qed.
 
-  lemma get_out (w:WB.t) i : 
-     !(0 <= i < r) => 
+  lemma get_out (w:WB.t) i :
+     !(0 <= i < r) =>
      w \bits'S i = WS.of_int 0.
   proof.
     move=> hi;apply WS.wordP => k hk.
-    rewrite bits'SiE 1:// WS.of_intwE /WS.int_bit /= get_to_uint. 
+    rewrite bits'SiE 1:// WS.of_intwE /WS.int_bit /= get_to_uint.
     smt(gt0_r WS.gt0_size sizeBrS).
   qed.
 
@@ -1085,9 +1580,9 @@ abstract theory W_WS.
     apply wordP => i hi; rewrite pack'RE initiE //= get_bits'S //.
     by rewrite get_unpack'S //;apply divz_cmp => //;rewrite -sizeBrS.
   qed.
-     
+
   lemma pack'RbE ws i : 0 <= i < r => pack'R_t ws \bits'S i = ws.[i].
-  proof. 
+  proof.
     move=> hr;apply WS.wordP => j hj.
     rewrite bits'SiE // pack'RE initiE /= ?in_bound //.
     by rewrite modzMDl divzMDl 1:/# divz_small ?modz_small; solve.
@@ -1105,32 +1600,32 @@ abstract theory W_WS.
   lemma allP (w1 w2 :WB.t) : all (fun i => w1 \bits'S i = w2 \bits'S i) (iota_ 0 r) => w1 = w2.
   proof. rewrite allP => h; apply wordP => i; rewrite -(mema_iota 0 r); apply h. qed.
 
-  abbrev map (f:WS.t -> WS.t) (w:WB.t) = 
+  abbrev map (f:WS.t -> WS.t) (w:WB.t) =
     pack'R_t (map f (unpack'S w)).
 
-  abbrev map2 (f:WS.t -> WS.t -> WS.t) (w1 w2:WB.t) = 
+  abbrev map2 (f:WS.t -> WS.t -> WS.t) (w1 w2:WB.t) =
     pack'R_t (map2 f (unpack'S w1) (unpack'S w2)).
 
-  lemma mapbE f w i : 0 <= i < r => 
+  lemma mapbE f w i : 0 <= i < r =>
     (map f w) \bits'S i = f (w \bits'S i).
   proof.
     by move=> hi;rewrite pack'RbE // mapiE // initiE.
   qed.
 
-  lemma map2bE f w1 w2 i : 0 <= i < r => 
+  lemma map2bE f w1 w2 i : 0 <= i < r =>
     (map2 f w1 w2) \bits'S i = f (w1 \bits'S i) (w2 \bits'S i).
   proof.
     by move=> hi;rewrite pack'RbE // map2iE // !initiE.
   qed.
 
-  lemma andb'SE (w1 w2:WB.t) i : 
+  lemma andb'SE (w1 w2:WB.t) i :
     (WB.andw w1 w2) \bits'S i = WS.andw (w1 \bits'S i) (w2 \bits'S i).
   proof.
     apply WS.wordP => j hj.
     by rewrite bits'SiE // WB.andwE WS.andwE !bits'SiE.
   qed.
 
-  lemma orb'SE (w1 w2:WB.t) i : 
+  lemma orb'SE (w1 w2:WB.t) i :
     (WB.orw w1 w2) \bits'S i = WS.orw (w1 \bits'S i) (w2 \bits'S i).
   proof.
     apply WS.wordP => j hj.
@@ -1149,35 +1644,36 @@ abstract theory W_WS.
     (WB.invw w) \bits'S i = WS.invw (w \bits'S i).
   proof.
     move=> hi;apply WS.wordP => j hj.
-    rewrite bits'SiE // WB.invwE WS.invwE !bits'SiE //; smt (in_bound).
+    rewrite bits'SiE // WB.invwE WS.invwE !bits'SiE //.
+    by rewrite in_bound /#.
   qed.
 
-  lemma andb'Ru'SE ws1 ws2 : 
+  lemma andb'Ru'SE ws1 ws2 :
     WB.andw (pack'R_t ws1) (pack'R_t ws2) = pack'R_t (map2 WS.andw ws1 ws2).
    proof.
      apply (canRL _ _ _ _ unpack'SK); apply packP => i hi.
-     by rewrite get_unpack'S // map2iE // andb'SE // !pack'RbE. 
+     by rewrite get_unpack'S // map2iE // andb'SE // !pack'RbE.
    qed.
 
-   lemma orb'Ru'SE ws1 ws2 : 
+   lemma orb'Ru'SE ws1 ws2 :
      WB.orw (pack'R_t ws1) (pack'R_t ws2) = pack'R_t (map2 WS.orw ws1 ws2).
    proof.
      apply (canRL _ _ _ _ unpack'SK); apply packP => i hi.
-     by rewrite get_unpack'S // map2iE // orb'SE // !pack'RbE. 
+     by rewrite get_unpack'S // map2iE // orb'SE // !pack'RbE.
    qed.
 
-   lemma xorb'Ru'SE ws1 ws2 : 
+   lemma xorb'Ru'SE ws1 ws2 :
      WB.(+^) (pack'R_t ws1) (pack'R_t ws2) = pack'R_t (map2 WS.(+^) ws1 ws2).
    proof.
      apply (canRL _ _ _ _ unpack'SK); apply packP => i hi.
-     by rewrite get_unpack'S // map2iE // xorb'SE // !pack'RbE. 
+     by rewrite get_unpack'S // map2iE // xorb'SE // !pack'RbE.
    qed.
 
-   lemma invw'Ru'SE ws : 
+   lemma invw'Ru'SE ws :
      WB.invw (pack'R_t ws) = pack'R_t (map WS.invw ws).
    proof.
      apply (canRL _ _ _ _ unpack'SK); apply packP => i hi.
-     by rewrite get_unpack'S // mapiE // invw'SE // !pack'RbE. 
+     by rewrite get_unpack'S // mapiE // invw'SE // !pack'RbE.
    qed.
 
    lemma bits'S_div (w:WB.t) i : 0 <= i =>
@@ -1191,9 +1687,9 @@ abstract theory W_WS.
 
    lemma of_int_bits'S_div w i : 0 <= i < r =>
      (WB.of_int w) \bits'S i = WS.of_int (w %/ (2^(sizeS*i))).
-   proof. 
+   proof.
      move=> [h0i hir];rewrite bits'S_div //.
-     rewrite WB.of_uintK modz_pow2_div. 
+     rewrite WB.of_uintK modz_pow2_div.
      + by rewrite sizeBrS mulzC; apply cmpW; apply mulz_cmp_r.
      rewrite -WS.of_int_mod modz_mod_pow2 /min.
      have -> /= : !sizeB - sizeS * i < sizeS.
@@ -1203,19 +1699,19 @@ abstract theory W_WS.
      by rewrite WS.of_int_mod.
    qed.
 
-   lemma of_int_bits'S_div_red (w i:int) : 0 <= i < r => 
+   lemma of_int_bits'S_div_red (w i:int) : 0 <= i < r =>
      0 <= `|w| => (* Do not remove this condition, it is used to block reduction *)
-     (WB.of_int w) \bits'S i = WS.of_int (w %/ (2^(sizeS*i))).  
+     (WB.of_int w) \bits'S i = WS.of_int (w %/ (2^(sizeS*i))).
    proof. by move=> hi hw;apply of_int_bits'S_div. qed.
- 
-   hint simplify (pack'RwE, bits'SiE, pack'RbE, get_unpack'S, unpack'SK, pack'RK, 
+
+   hint simplify (pack'RwE, bits'SiE, pack'RbE, get_unpack'S, unpack'SK, pack'RK,
                   mapbE, map2bE, andb'SE, orb'SE, xorb'SE, invw'SE,
                   andb'Ru'SE, orb'Ru'SE, xorb'Ru'SE, invw'Ru'SE, of_int_bits'S_div_red).
 
    lemma to_uint_zeroextu'B (w:WS.t) :
      WB.to_uint (zeroextu'B w) = WS.to_uint w.
    proof.
-     rewrite /zeroextu'B WB.of_uintK modz_small //. 
+     rewrite /zeroextu'B WB.of_uintK modz_small //.
      apply bound_abs;have [h1 h2] := WS.to_uint_cmp w;split => // ?.
      apply: (ltr_le_trans (2^sizeS)) => //.
      apply pow_Mle;smt (le_size WS.gt0_size).
@@ -1238,17 +1734,17 @@ abstract theory W_WS.
 
    lemma zeroext_truncateu'S_and (w:WB.t) :
      zeroextu'B (truncateu'S w) = andw w (WB.of_int (2^sizeS - 1)).
-   proof. 
+   proof.
      rewrite WB.and_mod; 1: smt (le_size WS.gt0_size).
      rewrite -(WB.to_uintK (zeroextu'B (truncateu'S w))).
-     by rewrite to_uint_zeroextu'B to_uint_truncateu'S. 
+     by rewrite to_uint_zeroextu'B to_uint_truncateu'S.
    qed.
 
-   lemma of_uint_pack'R i : 
-      (WB.of_int i) = 
+   lemma of_uint_pack'R i :
+      (WB.of_int i) =
         pack'R (map (fun k => WS.of_int ((i %/ 2^(sizeS * k)) %% 2^sizeS)) (iota_ 0 r)).
    proof.
-     rewrite -(unpack'SK (WB.of_int i)) /unpack'S Pack.init_of_list. 
+     rewrite -(unpack'SK (WB.of_int i)) /unpack'S Pack.init_of_list.
      do 2! congr; apply (eq_from_nth (WS.of_int 0)) => [ | k]; rewrite !size_map //.
      move=> hk;rewrite !(nth_map 0) //=.
      move: hk;rewrite size_iota /max gt0_r /= => hk;rewrite !nth_iota //=.
@@ -1262,25 +1758,25 @@ abstract theory W_WS.
      by move=> ?;apply ler_pemulr => // /#.
    qed.
 
-   op x86_VPADD_'Ru'S (w1 : WB.t) (w2:WB.t) = 
+   op x86_VPADD_'Ru'S (w1 : WB.t) (w2:WB.t) =
      map2 WS.(+) w1 w2.
 
-(*   op x86_VPSUB_'Ru'S (w1 : WB.t) (w2:WB.t) = 
+(*   op x86_VPSUB_'Ru'S (w1 : WB.t) (w2:WB.t) =
      map2 (fun (x y:WS.t) => x - y) w1 w2.
 
-   op x86_VPMUL_'Ru'S (w1 : WB.t) (w2:WB.t) = 
+   op x86_VPMUL_'Ru'S (w1 : WB.t) (w2:WB.t) =
      map2 WS.( * ) w1 w2. *)
 
-   op x86_VPSLL_'Ru'S (w : WB.t) (cnt : W8.t) = 
+   op x86_VPSLL_'Ru'S (w : WB.t) (cnt : W8.t) =
      map (fun (w:WS.t) => w `<<` cnt) w.
 
-   op x86_VPSRL_'Ru'S (w : WB.t) (cnt : W8.t) = 
+   op x86_VPSRL_'Ru'S (w : WB.t) (cnt : W8.t) =
      map (fun (w:WS.t) => w `>>` cnt) w.
 
-   op x86_VPBROADCAST_'Ru'S (w: WS.t) = 
+   op x86_VPBROADCAST_'Ru'S (w: WS.t) =
      pack'R (map (fun i => w) (iota_ 0 r)).
 
-   lemma x86_'Ru'S_rol_xor i w : 0 < i < sizeS => 
+   lemma x86_'Ru'S_rol_xor i w : 0 < i < sizeS =>
       x86_VPSLL_'Ru'S w (W8.of_int i) +^ x86_VPSRL_'Ru'S w (W8.of_int (sizeS - i)) =
       map (fun w0 => WS.rol w0 i) w.
    proof.
@@ -1289,7 +1785,7 @@ abstract theory W_WS.
      by rewrite xorb'SE !pack'RbE 1..3:// !mapiE 1..3:// /= rol_xor_shft.
    qed.
 
-   lemma x86_'Ru'S_rol_xor_red w1 w2 i si: 
+   lemma x86_'Ru'S_rol_xor_red w1 w2 i si:
      w1 = w2 => W8.to_uint si = sizeS - W8.to_uint i => 0 < W8.to_uint i < sizeS =>
      x86_VPSLL_'Ru'S w1 i +^ x86_VPSRL_'Ru'S w2 si =
      map (fun w0 => WS.rol w0 (W8.to_uint i)) w1.
@@ -1307,7 +1803,7 @@ abstract theory BitWordSH.
   clone include BitWord with op size <- size.
 
   op (`>>`) (w1 : t) (w2 : W8.t) = w1 `>>>` (to_uint w2 %% size).
-  op (`<<`) (w1 : t) (w2 : W8.t) = w1 `<<<` (to_uint w2 %% size). 
+  op (`<<`) (w1 : t) (w2 : W8.t) = w1 `<<<` (to_uint w2 %% size).
 
   lemma shr_div w1 w2 : to_uint (w1 `>>` w2) = to_uint w1 %/ 2^ (to_uint w2 %% size).
   proof.
@@ -1317,7 +1813,7 @@ abstract theory BitWordSH.
     by have:= to_uint_cmp w1; smt (gt0_pow2).
   qed.
 
-  lemma shr_div_le w1 i : 0 <= i < size => 
+  lemma shr_div_le w1 i : 0 <= i < size =>
      to_uint (w1 `>>` (W8.of_int i)) = to_uint w1 %/ 2^ i.
   proof.
     move=> hi;rewrite shr_div of_uintK.
@@ -1325,7 +1821,7 @@ abstract theory BitWordSH.
     by rewrite modz_small //;apply bound_abs.
   qed.
 
-  lemma rol_xor_shft w i : 0 < i < size => 
+  lemma rol_xor_shft w i : 0 < i < size =>
     rol w i = (w `<<` W8.of_int i) +^ (w `>>` W8.of_int (size - i)).
   proof.
     move=> hi; rewrite /(`<<`) /(`>>`) !W8.of_uintK.
@@ -1333,6 +1829,24 @@ abstract theory BitWordSH.
     + by rewrite /=; smt (size_le_256).
     rewrite !(modz_small _ W8.modulus) 1:// 1:[smt (size_le_256)] !modz_small 1,2:/#.
     by rewrite rol_xor 1:/#.
+  qed.
+
+  lemma shl_shlw k w:
+   0 <= k < size =>
+   w `<<` W8.of_int k = w `<<<` k.
+  proof.
+   move=> *; rewrite /(`<<`) of_uintK (modz_small (k %% W8.modulus)).
+    smt(modz_cmp).
+   by rewrite modz_small //; smt(size_le_256).
+  qed.
+
+  lemma shr_shrw k w:
+   0 <= k < size =>
+   w `>>` W8.of_int k = w `>>>` k.
+  proof.
+   move=> *; rewrite /(`>>`) of_uintK (modz_small (k %% W8.modulus)).
+    smt(modz_cmp).
+   by rewrite modz_small //; smt(size_le_256).
   qed.
 
 end BitWordSH.
@@ -1344,8 +1858,8 @@ theory W16.
         size_le_256 by done.
 end W16. export W16.
 
-clone export W_WS as W2u8 with 
-  op sizeS <- W8.size, op sizeB <- W16.size, op r <- 2, 
+clone export W_WS as W2u8 with
+  op sizeS <- W8.size, op sizeB <- W16.size, op r <- 2,
   theory WS <- W8, theory WB <- W16
   proof gt0_r by done, sizeBrS by done
   rename [op, lemma] "'Ru'S" as "2u8" "'R" as "2" "'S" as "8" "'B" as "16" .
@@ -1357,17 +1871,17 @@ theory W32.
         size_le_256 by done.
 end W32. export W32.
 
-clone export W_WS as W4u8 with 
-  op sizeS <- W8.size, op sizeB <- W32.size, op r <- 4, 
+clone export W_WS as W4u8 with
+  op sizeS <- W8.size, op sizeB <- W32.size, op r <- 4,
   theory WS <- W8, theory WB <- W32
   proof gt0_r by done, sizeBrS by done
-  rename [op, lemma] "'Ru'S" as "4u8" "'R" as "4" "'S" as "8" "'B" as "32". 
+  rename [op, lemma] "'Ru'S" as "4u8" "'R" as "4" "'S" as "8" "'B" as "32".
 
-clone export W_WS as W2u16 with 
-  op sizeS <- W16.size, op sizeB <- W32.size, op r <- 2, 
+clone export W_WS as W2u16 with
+  op sizeS <- W16.size, op sizeB <- W32.size, op r <- 2,
   theory WS <- W16, theory WB <- W32
   proof gt0_r by done, sizeBrS by done
-  rename [op, lemma] "'Ru'S" as "2u16" "'R" as "2" "'S" as "16" "'B" as "32". 
+  rename [op, lemma] "'Ru'S" as "2u16" "'R" as "2" "'S" as "16" "'B" as "32".
 
 theory W64.
   abbrev [-printing] size = 64.
@@ -1376,23 +1890,23 @@ theory W64.
         size_le_256 by done.
 end W64. export W64.
 
-clone export W_WS as W8u8 with 
-  op sizeS <- W8.size, op sizeB <- W64.size, op r <- 8, 
+clone export W_WS as W8u8 with
+  op sizeS <- W8.size, op sizeB <- W64.size, op r <- 8,
   theory WS <- W8, theory WB <- W64
   proof gt0_r by done, sizeBrS by done
-  rename [op, lemma] "'Ru'S" as "8u8" "'R" as "8" "'S" as "8" "'B" as "64". 
+  rename [op, lemma] "'Ru'S" as "8u8" "'R" as "8" "'S" as "8" "'B" as "64".
 
-clone export W_WS as W4u16 with 
-  op sizeS <- W16.size, op sizeB <- W64.size, op r <- 4, 
+clone export W_WS as W4u16 with
+  op sizeS <- W16.size, op sizeB <- W64.size, op r <- 4,
   theory WS <- W16, theory WB <- W64
   proof gt0_r by done, sizeBrS by done
-  rename [op, lemma] "'Ru'S" as "4u16" "'R" as "4" "'S" as "16" "'B" as "64". 
+  rename [op, lemma] "'Ru'S" as "4u16" "'R" as "4" "'S" as "16" "'B" as "64".
 
-clone export W_WS as W2u32 with 
-  op sizeS <- W32.size, op sizeB <- W64.size, op r <- 2, 
+clone export W_WS as W2u32 with
+  op sizeS <- W32.size, op sizeB <- W64.size, op r <- 2,
   theory WS <- W32, theory WB <- W64
   proof gt0_r by done, sizeBrS by done
-  rename [op, lemma] "'Ru'S" as "2u32" "'R" as "2" "'S" as "32" "'B" as "64". 
+  rename [op, lemma] "'Ru'S" as "2u32" "'R" as "2" "'S" as "32" "'B" as "64".
 
 theory W128.
   abbrev [-printing] size = 128.
@@ -1401,29 +1915,29 @@ theory W128.
         size_le_256 by done.
 end W128. export W128.
 
-clone export W_WS as W16u8 with 
-  op sizeS <- W8.size, op sizeB <- W128.size, op r <- 16, 
+clone export W_WS as W16u8 with
+  op sizeS <- W8.size, op sizeB <- W128.size, op r <- 16,
   theory WS <- W8, theory WB <- W128
   proof gt0_r by done, sizeBrS by done
-  rename [op, lemma] "'Ru'S" as "16u8" "'R" as "16" "'S" as "8" "'B" as "128". 
+  rename [op, lemma] "'Ru'S" as "16u8" "'R" as "16" "'S" as "8" "'B" as "128".
 
-clone export W_WS as W8u16 with 
-  op sizeS <- W16.size, op sizeB <- W128.size, op r <- 8, 
+clone export W_WS as W8u16 with
+  op sizeS <- W16.size, op sizeB <- W128.size, op r <- 8,
   theory WS <- W16, theory WB <- W128
   proof gt0_r by done, sizeBrS by done
-  rename [op, lemma] "'Ru'S" as "8u16" "'R" as "8" "'S" as "16" "'B" as "128". 
+  rename [op, lemma] "'Ru'S" as "8u16" "'R" as "8" "'S" as "16" "'B" as "128".
 
-clone export W_WS as W4u32 with 
-  op sizeS <- W32.size, op sizeB <- W128.size, op r <- 4, 
+clone export W_WS as W4u32 with
+  op sizeS <- W32.size, op sizeB <- W128.size, op r <- 4,
   theory WS <- W32, theory WB <- W128
   proof gt0_r by done, sizeBrS by done
-  rename [op, lemma] "'Ru'S" as "4u32" "'R" as "4" "'S" as "32" "'B" as "128". 
+  rename [op, lemma] "'Ru'S" as "4u32" "'R" as "4" "'S" as "32" "'B" as "128".
 
-clone export W_WS as W2u64 with 
-  op sizeS <- W64.size, op sizeB <- W128.size, op r <- 2, 
+clone export W_WS as W2u64 with
+  op sizeS <- W64.size, op sizeB <- W128.size, op r <- 2,
   theory WS <- W64, theory WB <- W128
   proof gt0_r by done, sizeBrS by done
-  rename [op, lemma] "'Ru'S" as "2u64" "'R" as "2" "'S" as "64" "'B" as "128". 
+  rename [op, lemma] "'Ru'S" as "2u64" "'R" as "2" "'S" as "64" "'B" as "128".
 
 theory W256.
   abbrev [-printing] size = 256.
@@ -1432,35 +1946,35 @@ theory W256.
         size_le_256 by done.
 end W256. export W256.
 
-clone export W_WS as W32u8 with 
-  op sizeS <- W8.size, op sizeB <- W256.size, op r <- 32, 
+clone export W_WS as W32u8 with
+  op sizeS <- W8.size, op sizeB <- W256.size, op r <- 32,
   theory WS <- W8, theory WB <- W256
   proof gt0_r by done, sizeBrS by done
-  rename [op, lemma] "'Ru'S" as "32u8" "'R" as "32" "'S" as "8" "'B" as "256". 
+  rename [op, lemma] "'Ru'S" as "32u8" "'R" as "32" "'S" as "8" "'B" as "256".
 
-clone export W_WS as W16u16 with 
-  op sizeS <- W16.size, op sizeB <- W256.size, op r <- 16, 
+clone export W_WS as W16u16 with
+  op sizeS <- W16.size, op sizeB <- W256.size, op r <- 16,
   theory WS <- W16, theory WB <- W256
   proof gt0_r by done, sizeBrS by done
-  rename [op, lemma] "'Ru'S" as "16u16" "'R" as "16" "'S" as "16" "'B" as "256". 
+  rename [op, lemma] "'Ru'S" as "16u16" "'R" as "16" "'S" as "16" "'B" as "256".
 
-clone export W_WS as W8u32 with 
-  op sizeS <- W32.size, op sizeB <- W256.size, op r <- 8, 
+clone export W_WS as W8u32 with
+  op sizeS <- W32.size, op sizeB <- W256.size, op r <- 8,
   theory WS <- W32, theory WB <- W256
   proof gt0_r by done, sizeBrS by done
-  rename [op, lemma] "'Ru'S" as "8u32" "'R" as "8" "'S" as "32" "'B" as "256". 
+  rename [op, lemma] "'Ru'S" as "8u32" "'R" as "8" "'S" as "32" "'B" as "256".
 
-clone export W_WS as W4u64 with 
-  op sizeS <- W64.size, op sizeB <- W256.size, op r <- 4, 
+clone export W_WS as W4u64 with
+  op sizeS <- W64.size, op sizeB <- W256.size, op r <- 4,
   theory WS <- W64, theory WB <- W256
   proof gt0_r by done, sizeBrS by done
-  rename [op, lemma] "'Ru'S" as "4u64" "'R" as "4" "'S" as "64" "'B" as "256". 
+  rename [op, lemma] "'Ru'S" as "4u64" "'R" as "4" "'S" as "64" "'B" as "256".
 
-clone export W_WS as W2u128 with 
-  op sizeS <- W128.size, op sizeB <- W256.size, op r <- 2, 
+clone export W_WS as W2u128 with
+  op sizeS <- W128.size, op sizeB <- W256.size, op r <- 2,
   theory WS <- W128, theory WB <- W256
   proof gt0_r by done, sizeBrS by done
-  rename [op, lemma] "'Ru'S" as "2u128" "'R" as "2" "'S" as "128" "'B" as "256". 
+  rename [op, lemma] "'Ru'S" as "2u128" "'R" as "2" "'S" as "128" "'B" as "256".
 
 
 (* -------------------------------------------------------------------- *)
@@ -1475,7 +1989,7 @@ type wsize = [
   | W256
 ].
 
-op wsize_i (w:wsize) = 
+op wsize_i (w:wsize) =
   with w = W8   => 1
   with w = W16  => 2
   with w = W32  => 4
@@ -1502,12 +2016,12 @@ lemma foo (x y:W128.t) (x1 x2 y1 y2:W64.t):
   map2 W64.( + ) x y = pack2 [x1 + y1; x2 + y2].
 proof. by move=> -> -> /=. qed.
 
-op bits_eq (w:W128.t) xs = 
-  all (fun (ix:int * W64.t) => w \bits64 ix.`1 = ix.`2) 
+op bits_eq (w:W128.t) xs =
+  all (fun (ix:int * W64.t) => w \bits64 ix.`1 = ix.`2)
     (zip (iota_ 0 (size xs)) xs).
 
 lemma foo1 (x y:W128.t) (x0 x1 y0 y1:W64.t):
-   (bits_eq x [x0; x1]) => 
+   (bits_eq x [x0; x1]) =>
    (bits_eq y [y0; y1]) =>
    (bits_eq (map2 W64.( + ) x y) [x0 + y0; x1 + y1]).
 proof. rewrite /bits_eq /= => />. qed.
@@ -1519,9 +2033,9 @@ lemma foo (x y:W128.t) (x1 x2 y1 y2:W64.t):
 proof. move=> -> -> /=.
 *)
 
-lemma divmod_mul n d i j : 
-  0 < n => 
-  0 <= j < d =>  
+lemma divmod_mul n d i j :
+  0 < n =>
+  0 <= j < d =>
   (i * d + j) %/ (n * d) = i%/ n /\ (i * d + j) %% (n * d) = i %% n * d + j.
 proof.
   move=> hn hj.
@@ -1529,11 +2043,11 @@ proof.
   + have [h1 h2]:= edivzP i n.
     by rewrite {1 2} h1 divzMDl 1:/# (divz_small (i%%n) n) 1:/# /=; ring.
   rewrite divzMDl 1:/# modzMDl.
-  have hb: 0 <= d * (i %% n) + j < `|n * d|. 
+  have hb: 0 <= d * (i %% n) + j < `|n * d|.
   + have := modz_cmp i n hn.
     have -> : `|n * d| = n * d by smt().
     have -> h : n * d = (n-1) * d + d by ring.
-    split;1: smt(); move=> ?. 
+    split;1: smt(); move=> ?.
     apply ler_lt_add; 2:smt().
     by rewrite mulzC ler_pmul2r /#.
   by rewrite (divz_small _ (n*d)) 1://  (modz_small _ (n*d)) 1:// /=; ring.
@@ -1543,129 +2057,129 @@ qed.
 (* Lemmas on \bits8                                                                  *)
 (* --------------------------------------------------------------------------------- *)
 
-lemma bits8_W2u16 ws i : 
+lemma bits8_W2u16 ws i :
   W2u16.pack2_t ws \bits8 i = if 0 <= i < 4 then ws.[i%/2] \bits8 (i%%2) else W8.zero.
 proof.
-  apply W8.wordP => j hj; rewrite !bits8iE 1,2://. 
+  apply W8.wordP => j hj; rewrite !bits8iE 1,2://.
   case: (0 <= i < 4) => /= hi; last by rewrite W32.get_out 1:/#.
   rewrite pack2wE 1:/#; have /= [-> ->] := divmod_mul 2 8 i j _ hj; 1 :done; rewrite W2u8.bits8iE 1:// /#.
 qed.
 
-lemma bits8_W2u16_red ws i : 
+lemma bits8_W2u16_red ws i :
   0 <= i < 4 => W2u16.pack2_t ws \bits8 i = ws.[i%/2] \bits8 (i%%2).
 proof. by move=> h;rewrite bits8_W2u16 h. qed.
 
-lemma bits8_W4u16 ws i : 
+lemma bits8_W4u16 ws i :
   W4u16.pack4_t ws \bits8 i = if 0 <= i < 8 then ws.[i%/2] \bits8 (i%%2) else W8.zero.
 proof.
-  apply W8.wordP => j hj; rewrite !bits8iE 1,2://. 
+  apply W8.wordP => j hj; rewrite !bits8iE 1,2://.
   case: (0 <= i < 8) => /= hi; last by rewrite W64.get_out 1:/#.
   rewrite pack4wE 1:/#; have /= [-> ->] := divmod_mul 2 8 i j _ hj; 1:done; rewrite W2u8.bits8iE 1:// /#.
 qed.
 
-lemma bits8_W4u16_red ws i : 
+lemma bits8_W4u16_red ws i :
   0 <= i < 8 => W4u16.pack4_t ws \bits8 i = ws.[i%/2] \bits8 (i%%2).
 proof. by move=> h;rewrite bits8_W4u16 h. qed.
 
-lemma bits8_W8u16 ws i : 
+lemma bits8_W8u16 ws i :
   W8u16.pack8_t ws \bits8 i = if 0 <= i < 16 then ws.[i%/2] \bits8 (i%%2) else W8.zero.
 proof.
-  apply W8.wordP => j hj; rewrite !bits8iE 1,2://. 
+  apply W8.wordP => j hj; rewrite !bits8iE 1,2://.
   case: (0 <= i < 16) => /= hi; last by rewrite W128.get_out 1:/#.
   rewrite pack8wE 1:/#; have [-> ->] := divmod_mul 2 8 i j _ hj; 1: done; rewrite W2u8.bits8iE 1:// /#.
 qed.
 
-lemma bits8_W8u16_red ws i : 
+lemma bits8_W8u16_red ws i :
   0 <= i < 16 => W8u16.pack8_t ws \bits8 i = ws.[i%/2] \bits8 (i%%2).
 proof. by move=> h;rewrite bits8_W8u16 h. qed.
 
-lemma bits8_W16u16 ws i : 
+lemma bits8_W16u16 ws i :
   W16u16.pack16_t ws \bits8 i = if 0 <= i < 32 then ws.[i%/2] \bits8 (i%%2) else W8.zero.
 proof.
-  apply W8.wordP => j hj; rewrite !bits8iE 1,2://. 
+  apply W8.wordP => j hj; rewrite !bits8iE 1,2://.
   case: (0 <= i < 32) => /= hi; last by rewrite W256.get_out 1:/#.
   rewrite pack16wE 1:/#; have [-> ->] := divmod_mul 2 8 i j _ hj; 1: done; rewrite W2u8.bits8iE 1:// /#.
 qed.
 
-lemma bits8_W16u16_red ws i : 
+lemma bits8_W16u16_red ws i :
   0 <= i < 32 => W16u16.pack16_t ws \bits8 i = ws.[i%/2] \bits8 (i%%2).
 proof. by move=> h;rewrite bits8_W16u16 h. qed.
 
 hint simplify bits8_W2u16_red, bits8_W4u16_red, bits8_W8u16_red, bits8_W16u16_red.
 
-lemma bits8_W2u32 ws i : 
+lemma bits8_W2u32 ws i :
   W2u32.pack2_t ws \bits8 i = if 0 <= i < 8 then ws.[i%/4] \bits8 (i%%4) else W8.zero.
 proof.
-  apply W8.wordP => j hj; rewrite !bits8iE 1,2://. 
+  apply W8.wordP => j hj; rewrite !bits8iE 1,2://.
   case: (0 <= i < 8) => /= hi; last by rewrite W64.get_out 1:/#.
   rewrite pack2wE 1:/#; have /= [-> ->] := divmod_mul 4 8 i j _ hj; 1: done; rewrite W4u8.bits8iE 1:// /#.
 qed.
 
-lemma bits8_W2u32_red ws i : 
+lemma bits8_W2u32_red ws i :
   0 <= i < 8 => W2u32.pack2_t ws \bits8 i = ws.[i%/4] \bits8 (i%%4).
 proof. by move=> h;rewrite bits8_W2u32 h. qed.
 
-lemma bits8_W4u32 ws i : 
+lemma bits8_W4u32 ws i :
   W4u32.pack4_t ws \bits8 i = if 0 <= i < 16 then ws.[i%/4] \bits8 (i%%4) else W8.zero.
 proof.
-  apply W8.wordP => j hj; rewrite !bits8iE 1,2://. 
+  apply W8.wordP => j hj; rewrite !bits8iE 1,2://.
   case: (0 <= i < 16) => /= hi; last by rewrite W128.get_out 1:/#.
   rewrite pack4wE 1:/#; have /= [-> ->] := divmod_mul 4 8 i j _ hj; 1: done; rewrite W4u8.bits8iE 1:// /#.
 qed.
 
-lemma bits8_W4u32_red ws i : 
+lemma bits8_W4u32_red ws i :
   0 <= i < 16 => W4u32.pack4_t ws \bits8 i = ws.[i%/4] \bits8 (i%%4).
 proof. by move=> h;rewrite bits8_W4u32 h. qed.
 
-lemma bits8_W8u32 ws i : 
+lemma bits8_W8u32 ws i :
   W8u32.pack8_t ws \bits8 i = if 0 <= i < 32 then ws.[i%/4] \bits8 (i%%4) else W8.zero.
 proof.
-  apply W8.wordP => j hj; rewrite !bits8iE 1,2://. 
+  apply W8.wordP => j hj; rewrite !bits8iE 1,2://.
   case: (0 <= i < 32) => /= hi; last by rewrite W256.get_out 1:/#.
   rewrite pack8wE 1:/#; have /= [-> ->] := divmod_mul 4 8 i j _ hj; 1: done; rewrite W4u8.bits8iE 1:// /#.
 qed.
 
-lemma bits8_W8u32_red ws i : 
+lemma bits8_W8u32_red ws i :
   0 <= i < 32 => W8u32.pack8_t ws \bits8 i = ws.[i%/4] \bits8 (i%%4).
 proof. by move=> h;rewrite bits8_W8u32 h. qed.
 
 hint simplify bits8_W2u32_red, bits8_W4u32_red, bits8_W8u32_red.
 
-lemma bits8_W2u64 ws i : 
+lemma bits8_W2u64 ws i :
   W2u64.pack2_t ws \bits8 i = if 0 <= i < 16 then ws.[i%/8] \bits8 (i%%8) else W8.zero.
 proof.
-  apply W8.wordP => j hj; rewrite !bits8iE 1,2://. 
+  apply W8.wordP => j hj; rewrite !bits8iE 1,2://.
   case: (0 <= i < 16) => /= hi; last by rewrite W128.get_out 1:/#.
   rewrite pack2wE 1:/#; have /= [-> ->] := divmod_mul 8 8 i j _ hj; 1: done; rewrite W8u8.bits8iE 1:// /#.
 qed.
 
-lemma bits8_W2u64_red ws i : 
+lemma bits8_W2u64_red ws i :
   0 <= i < 16 => W2u64.pack2_t ws \bits8 i = ws.[i%/8] \bits8 (i%%8).
 proof. by move=> h;rewrite bits8_W2u64 h. qed.
 
-lemma bits8_W4u64 ws i : 
+lemma bits8_W4u64 ws i :
   W4u64.pack4_t ws \bits8 i = if 0 <= i < 32 then ws.[i%/8] \bits8 (i%%8) else W8.zero.
 proof.
-  apply W8.wordP => j hj; rewrite !bits8iE 1,2://. 
+  apply W8.wordP => j hj; rewrite !bits8iE 1,2://.
   case: (0 <= i < 32) => /= hi; last by rewrite W256.get_out 1:/#.
   rewrite pack4wE 1:/#; have /= [-> ->] := divmod_mul 8 8 i j _ hj; 1: done; rewrite W8u8.bits8iE 1:// /#.
 qed.
 
-lemma bits8_W4u64_red ws i : 
+lemma bits8_W4u64_red ws i :
   0 <= i < 32 => W4u64.pack4_t ws \bits8 i = ws.[i%/8] \bits8 (i%%8).
 proof. by move=> h;rewrite bits8_W4u64 h. qed.
 
 hint simplify bits8_W2u64_red, bits8_W4u64_red.
 
-lemma bits8_W2u128 ws i : 
+lemma bits8_W2u128 ws i :
   W2u128.pack2_t ws \bits8 i = if 0 <= i < 32 then ws.[i%/16] \bits8 (i%%16) else W8.zero.
 proof.
-  apply W8.wordP => j hj; rewrite !bits8iE 1,2://. 
+  apply W8.wordP => j hj; rewrite !bits8iE 1,2://.
   case: (0 <= i < 32) => /= hi; last by rewrite W256.get_out 1:/#.
   rewrite pack2wE 1:/#; have /= [-> ->] := divmod_mul 16 8 i j _ hj; 1: done; rewrite W16u8.bits8iE 1:// /#.
 qed.
 
-lemma bits8_W2u128_red ws i : 
+lemma bits8_W2u128_red ws i :
   0 <= i < 32 => W2u128.pack2_t ws \bits8 i = ws.[i%/16] \bits8 (i%%16).
 proof. by move=> h;rewrite bits8_W2u128 h. qed.
 
@@ -1716,7 +2230,7 @@ proof.
 qed.
 
 hint simplify W64_bits32_bits8, W128_bits32_bits8, W256_bits32_bits8.
- 
+
 lemma W128_bits64_bits8 (w:W128.t) i j: 0 <= j < 8 => w \bits64 i \bits8 j = w \bits8 (8 * i + j).
 proof.
   move=> hj; apply W8.wordP => k hk.
@@ -1742,8 +2256,8 @@ hint simplify W256_bits128_bits8.
 (* --------------------------------------------------------------------------------- *)
 (* Lemmas on \bits16                                                                  *)
 (* --------------------------------------------------------------------------------- *)
-  
-lemma bits16_W4u8 ws i : 
+
+lemma bits16_W4u8 ws i :
   W4u8.pack4_t ws \bits16 i = if 0 <= i < 2 then W2u8.pack2 [ws.[2 * i]; ws.[2 * i + 1]] else W16.zero.
 proof.
   apply W2u8.wordP => j hj.
@@ -1753,11 +2267,11 @@ proof.
   by have []-> : j = 0 \/ j = 1 by smt().
 qed.
 
-lemma bits16_W4u8_red ws i : 
+lemma bits16_W4u8_red ws i :
   0 <= i < 2 => W4u8.pack4_t ws \bits16 i = W2u8.pack2 [ws.[2 * i]; ws.[2 * i + 1]].
 proof. by move=> h;rewrite bits16_W4u8 h. qed.
 
-lemma bits16_W8u8 ws i : 
+lemma bits16_W8u8 ws i :
   W8u8.pack8_t ws \bits16 i = if 0 <= i < 4 then W2u8.pack2 [ws.[2 * i]; ws.[2 * i + 1]] else W16.zero.
 proof.
   apply W2u8.wordP => j hj.
@@ -1767,11 +2281,11 @@ proof.
   have []-> //: j = 0 \/ j = 1 by smt().
 qed.
 
-lemma bits16_W8u8_red ws i : 
+lemma bits16_W8u8_red ws i :
   0 <= i < 4 => W8u8.pack8_t ws \bits16 i = W2u8.pack2 [ws.[2 * i]; ws.[2 * i + 1]].
 proof. by move=> h;rewrite bits16_W8u8 h. qed.
 
-lemma bits16_W16u8 ws i : 
+lemma bits16_W16u8 ws i :
   W16u8.pack16_t ws \bits16 i = if 0 <= i < 8 then W2u8.pack2 [ws.[2 * i]; ws.[2 * i + 1]] else W16.zero.
 proof.
   apply W2u8.wordP => j hj.
@@ -1781,11 +2295,11 @@ proof.
   have []-> //: j = 0 \/ j = 1 by smt().
 qed.
 
-lemma bits16_W16u8_red ws i : 
+lemma bits16_W16u8_red ws i :
   0 <= i < 8 => W16u8.pack16_t ws \bits16 i = W2u8.pack2 [ws.[2 * i]; ws.[2 * i + 1]].
 proof. by move=> h;rewrite bits16_W16u8 h. qed.
 
-lemma bits16_W32u8 ws i : 
+lemma bits16_W32u8 ws i :
   W32u8.pack32_t ws \bits16 i = if 0 <= i < 16 then W2u8.pack2 [ws.[2 * i]; ws.[2 * i + 1]] else W16.zero.
 proof.
   apply W2u8.wordP => j hj.
@@ -1795,85 +2309,85 @@ proof.
   have []-> //: j = 0 \/ j = 1 by smt().
 qed.
 
-lemma bits16_W32u8_red ws i : 
+lemma bits16_W32u8_red ws i :
   0 <= i < 16 => W32u8.pack32_t ws \bits16 i = W2u8.pack2 [ws.[2 * i]; ws.[2 * i + 1]].
 proof. by move=> h;rewrite bits16_W32u8 h. qed.
 
 hint simplify bits16_W4u8_red, bits16_W8u8_red, bits16_W16u8_red, bits16_W32u8.
 
-lemma bits16_W2u32 ws i : 
+lemma bits16_W2u32 ws i :
   W2u32.pack2_t ws \bits16 i = if 0 <= i < 4 then ws.[i%/2] \bits16 (i%%2) else W16.zero.
 proof.
-  apply W16.wordP => j hj; rewrite !bits16iE 1,2://. 
+  apply W16.wordP => j hj; rewrite !bits16iE 1,2://.
   case: (0 <= i < 4) => /= hi; last by rewrite W64.get_out 1:/#.
   rewrite pack2wE 1:/#; have /= [-> ->] := divmod_mul 2 16 i j _ hj; 1: done; rewrite W2u16.bits16iE 1:// /#.
 qed.
 
-lemma bits16_W2u32_red ws i : 
+lemma bits16_W2u32_red ws i :
   0 <= i < 4 => W2u32.pack2_t ws \bits16 i = ws.[i%/2] \bits16 (i%%2).
 proof. by move=> h;rewrite bits16_W2u32 h. qed.
 
-lemma bits16_W4u32 ws i : 
+lemma bits16_W4u32 ws i :
   W4u32.pack4_t ws \bits16 i = if 0 <= i < 8 then ws.[i%/2] \bits16 (i%%2) else W16.zero.
 proof.
-  apply W16.wordP => j hj; rewrite !bits16iE 1,2://. 
+  apply W16.wordP => j hj; rewrite !bits16iE 1,2://.
   case: (0 <= i < 8) => /= hi; last by rewrite W128.get_out 1:/#.
   rewrite pack4wE 1:/#; have /= [-> ->] := divmod_mul 2 16 i j _ hj; 1: done; rewrite W2u16.bits16iE 1:// /#.
 qed.
 
-lemma bits16_W4u32_red ws i : 
+lemma bits16_W4u32_red ws i :
   0 <= i < 8 => W4u32.pack4_t ws \bits16 i = ws.[i%/2] \bits16 (i%%2).
 proof. by move=> h;rewrite bits16_W4u32 h. qed.
 
-lemma bits16_W8u32 ws i : 
+lemma bits16_W8u32 ws i :
   W8u32.pack8_t ws \bits16 i = if 0 <= i < 16 then ws.[i%/2] \bits16 (i%%2) else W16.zero.
 proof.
-  apply W16.wordP => j hj; rewrite !bits16iE 1,2://. 
+  apply W16.wordP => j hj; rewrite !bits16iE 1,2://.
   case: (0 <= i < 16) => /= hi; last by rewrite W256.get_out 1:/#.
   rewrite pack8wE 1:/#; have /= [-> ->] := divmod_mul 2 16 i j _ hj; 1: done; rewrite W2u16.bits16iE 1:// /#.
 qed.
 
-lemma bits16_W8u32_red ws i : 
+lemma bits16_W8u32_red ws i :
   0 <= i < 16 => W8u32.pack8_t ws \bits16 i = ws.[i%/2] \bits16 (i%%2).
 proof. by move=> h;rewrite bits16_W8u32 h. qed.
-  
+
 hint simplify bits16_W2u32_red, bits16_W4u32_red, bits16_W8u32_red.
 
-lemma bits16_W2u64 ws i : 
+lemma bits16_W2u64 ws i :
   W2u64.pack2_t ws \bits16 i = if 0 <= i < 8 then ws.[i%/4] \bits16 (i%%4) else W16.zero.
 proof.
-  apply W16.wordP => j hj; rewrite !bits16iE 1,2://. 
+  apply W16.wordP => j hj; rewrite !bits16iE 1,2://.
   case: (0 <= i < 8) => /= hi; last by rewrite W128.get_out 1:/#.
   rewrite pack2wE 1:/#; have /= [-> ->] := divmod_mul 4 16 i j _ hj; 1: done; rewrite W4u16.bits16iE 1:// /#.
 qed.
 
-lemma bits16_W2u64_red ws i : 
+lemma bits16_W2u64_red ws i :
   0 <= i < 8 => W2u64.pack2_t ws \bits16 i = ws.[i%/4] \bits16 (i%%4).
 proof. by move=> h;rewrite bits16_W2u64 h. qed.
 
-lemma bits16_W4u64 ws i : 
+lemma bits16_W4u64 ws i :
   W4u64.pack4_t ws \bits16 i = if 0 <= i < 16 then ws.[i%/4] \bits16 (i%%4) else W16.zero.
 proof.
-  apply W16.wordP => j hj; rewrite !bits16iE 1,2://. 
+  apply W16.wordP => j hj; rewrite !bits16iE 1,2://.
   case: (0 <= i < 16) => /= hi; last by rewrite W256.get_out 1:/#.
   rewrite pack4wE 1:/#; have /= [-> ->] := divmod_mul 4 16 i j _ hj; 1: done; rewrite W4u16.bits16iE 1:// /#.
 qed.
 
-lemma bits16_W4u64_red ws i : 
+lemma bits16_W4u64_red ws i :
   0 <= i < 16 => W4u64.pack4_t ws \bits16 i = ws.[i%/4] \bits16 (i%%4).
 proof. by move=> h;rewrite bits16_W4u64 h. qed.
 
 hint simplify bits16_W2u64_red, bits16_W4u64_red.
 
-lemma bits16_W2u128 ws i : 
+lemma bits16_W2u128 ws i :
   W2u128.pack2_t ws \bits16 i = if 0 <= i < 16 then ws.[i%/8] \bits16 (i%%8) else W16.zero.
 proof.
-  apply W16.wordP => j hj; rewrite !bits16iE 1,2://. 
+  apply W16.wordP => j hj; rewrite !bits16iE 1,2://.
   case: (0 <= i < 16) => /= hi; last by rewrite W256.get_out 1:/#.
   rewrite pack2wE 1:/#; have /= [-> ->] := divmod_mul 8 16 i j _ hj; 1: done; rewrite W8u16.bits16iE 1:// /#.
 qed.
 
-lemma bits16_W2u128_red ws i : 
+lemma bits16_W2u128_red ws i :
   0 <= i < 16 => W2u128.pack2_t ws \bits16 i = ws.[i%/8] \bits16 (i%%8).
 proof.  by move=> h;rewrite bits16_W2u128 h. qed.
 
@@ -1897,7 +2411,7 @@ proof.
   by rewrite !bits16iE 1,2:// bits32iE 1:/#; congr; ring.
 qed.
 
-hint simplify W64_bits32_bits16, W128_bits32_bits16, W256_bits32_bits16. 
+hint simplify W64_bits32_bits16, W128_bits32_bits16, W256_bits32_bits16.
 
 lemma W128_bits64_bits16 (w:W128.t) i j: 0 <= j < 4 => w \bits64 i \bits16 j = w \bits16 (4 * i + j).
 proof.
@@ -1922,9 +2436,9 @@ hint simplify W128_bits64_bits16, W256_bits64_bits16, W256_bits128_bits16.
 (* --------------------------------------------------------------------------------- *)
 (* Lemmas on \bits32                                                                  *)
 (* --------------------------------------------------------------------------------- *)
-  
-lemma bits32_W8u8 ws i : 
-  W8u8.pack8_t ws \bits32 i = 
+
+lemma bits32_W8u8 ws i :
+  W8u8.pack8_t ws \bits32 i =
     if 0 <= i < 2 then W4u8.pack4 [ws.[4 * i]; ws.[4 * i + 1]; ws.[4 * i + 2]; ws.[4 * i + 3] ] else W32.zero.
 proof.
   apply W4u8.wordP => j hj.
@@ -1934,14 +2448,14 @@ proof.
   by have [|[|[|]]]-> : j = 0 \/ j = 1 \/ j = 2 \/ j = 3 by smt().
 qed.
 
-lemma bits32_W8u8_red ws i : 
+lemma bits32_W8u8_red ws i :
   0 <= i < 2 =>
-  W8u8.pack8_t ws \bits32 i = 
+  W8u8.pack8_t ws \bits32 i =
     W4u8.pack4 [ws.[4 * i]; ws.[4 * i + 1]; ws.[4 * i + 2]; ws.[4 * i + 3] ].
 proof. by move=> h;rewrite bits32_W8u8 h. qed.
 
-lemma bits32_W16u8 ws i : 
-  W16u8.pack16_t ws \bits32 i = 
+lemma bits32_W16u8 ws i :
+  W16u8.pack16_t ws \bits32 i =
     if 0 <= i < 4 then W4u8.pack4 [ws.[4 * i]; ws.[4 * i + 1]; ws.[4 * i + 2]; ws.[4 * i + 3] ] else W32.zero.
 proof.
   apply W4u8.wordP => j hj.
@@ -1951,14 +2465,14 @@ proof.
   by have [|[|[|]]]-> : j = 0 \/ j = 1 \/ j = 2 \/ j = 3 by smt().
 qed.
 
-lemma bits32_W16u8_red ws i : 
+lemma bits32_W16u8_red ws i :
   0 <= i < 4 =>
-  W16u8.pack16_t ws \bits32 i = 
+  W16u8.pack16_t ws \bits32 i =
     W4u8.pack4 [ws.[4 * i]; ws.[4 * i + 1]; ws.[4 * i + 2]; ws.[4 * i + 3] ].
 proof. by move=> h;rewrite bits32_W16u8 h. qed.
 
-lemma bits32_W32u8 ws i : 
-  W32u8.pack32_t ws \bits32 i = 
+lemma bits32_W32u8 ws i :
+  W32u8.pack32_t ws \bits32 i =
     if 0 <= i < 8 then W4u8.pack4 [ws.[4 * i]; ws.[4 * i + 1]; ws.[4 * i + 2]; ws.[4 * i + 3] ] else W32.zero.
 proof.
   apply W4u8.wordP => j hj.
@@ -1968,16 +2482,16 @@ proof.
   by have [|[|[|]]]-> : j = 0 \/ j = 1 \/ j = 2 \/ j = 3 by smt().
 qed.
 
-lemma bits32_W32u8_red ws i : 
+lemma bits32_W32u8_red ws i :
   0 <= i < 8 =>
-  W32u8.pack32_t ws \bits32 i = 
+  W32u8.pack32_t ws \bits32 i =
     W4u8.pack4 [ws.[4 * i]; ws.[4 * i + 1]; ws.[4 * i + 2]; ws.[4 * i + 3] ].
 proof. by move=> h;rewrite bits32_W32u8 h. qed.
 
 hint simplify bits32_W8u8_red, bits32_W16u8_red, bits32_W32u8_red.
 
-lemma bits32_W4u16 ws i : 
-  W4u16.pack4_t ws \bits32 i = 
+lemma bits32_W4u16 ws i :
+  W4u16.pack4_t ws \bits32 i =
     if 0 <= i < 2 then W2u16.pack2 [ws.[2 * i]; ws.[2 * i + 1]] else W32.zero.
 proof.
   apply W2u16.wordP => j hj.
@@ -1987,13 +2501,13 @@ proof.
   by have []-> : j = 0 \/ j = 1 by smt().
 qed.
 
-lemma bits32_W4u16_red ws i : 
-  0 <= i < 2 => 
+lemma bits32_W4u16_red ws i :
+  0 <= i < 2 =>
   W4u16.pack4_t ws \bits32 i = W2u16.pack2 [ws.[2 * i]; ws.[2 * i + 1]].
 proof. by move=> h;rewrite bits32_W4u16 h. qed.
 
-lemma bits32_W8u16 ws i : 
-  W8u16.pack8_t ws \bits32 i = 
+lemma bits32_W8u16 ws i :
+  W8u16.pack8_t ws \bits32 i =
     if 0 <= i < 4 then W2u16.pack2 [ws.[2 * i]; ws.[2 * i + 1]] else W32.zero.
 proof.
   apply W2u16.wordP => j hj.
@@ -2003,13 +2517,13 @@ proof.
   by have []-> : j = 0 \/ j = 1 by smt().
 qed.
 
-lemma bits32_W8u16_red ws i : 
+lemma bits32_W8u16_red ws i :
   0 <= i < 4 =>
   W8u16.pack8_t ws \bits32 i = W2u16.pack2 [ws.[2 * i]; ws.[2 * i + 1]].
 proof. by move=> h;rewrite bits32_W8u16 h. qed.
 
-lemma bits32_W16u16 ws i : 
-  W16u16.pack16_t ws \bits32 i = 
+lemma bits32_W16u16 ws i :
+  W16u16.pack16_t ws \bits32 i =
     if 0 <= i < 8 then W2u16.pack2 [ws.[2 * i]; ws.[2 * i + 1]] else W32.zero.
 proof.
   apply W2u16.wordP => j hj.
@@ -2019,8 +2533,8 @@ proof.
   by have []-> : j = 0 \/ j = 1 by smt().
 qed.
 
-lemma bits32_W16u16_red ws i : 
-  0 <= i < 8 => 
+lemma bits32_W16u16_red ws i :
+  0 <= i < 8 =>
   W16u16.pack16_t ws \bits32 i = W2u16.pack2 [ws.[2 * i]; ws.[2 * i + 1]].
 proof. by move=> h;rewrite bits32_W16u16 h. qed.
 
@@ -2029,7 +2543,7 @@ hint simplify bits32_W4u16_red, bits32_W8u16_red, bits32_W16u16_red.
 lemma bits32_W2u64 ws i :
   W2u64.pack2_t ws \bits32 i = if 0 <= i < 4 then ws.[i%/2] \bits32 (i%%2) else W32.zero.
 proof.
-  apply W32.wordP => j hj; rewrite !bits32iE 1,2://. 
+  apply W32.wordP => j hj; rewrite !bits32iE 1,2://.
   case: (0 <= i < 4) => /= hi; last by rewrite W128.get_out 1:/#.
   rewrite pack2wE 1:/#; have /= [-> ->] := divmod_mul 2 32 i j _ hj; 1: done; rewrite W2u32.bits32iE 1:// /#.
 qed.
@@ -2041,7 +2555,7 @@ proof. by move=> h;rewrite bits32_W2u64 h. qed.
 lemma bits32_W4u64 ws i :
   W4u64.pack4_t ws \bits32 i = if 0 <= i < 8 then ws.[i%/2] \bits32 (i%%2) else W32.zero.
 proof.
-  apply W32.wordP => j hj; rewrite !bits32iE 1,2://. 
+  apply W32.wordP => j hj; rewrite !bits32iE 1,2://.
   case: (0 <= i < 8) => /= hi; last by rewrite W256.get_out 1:/#.
   rewrite pack4wE 1:/#; have /= [-> ->] := divmod_mul 2 32 i j _ hj; 1: done; rewrite W2u32.bits32iE 1:// /#.
 qed.
@@ -2055,7 +2569,7 @@ hint simplify bits32_W2u64_red, bits32_W4u64_red.
 lemma bits32_W2u128 ws i :
   W2u128.pack2_t ws \bits32 i = if 0 <= i < 8 then ws.[i%/4] \bits32 (i%%4) else W32.zero.
 proof.
-  apply W32.wordP => j hj; rewrite !bits32iE 1,2://. 
+  apply W32.wordP => j hj; rewrite !bits32iE 1,2://.
   case: (0 <= i < 8) => /= hi; last by rewrite W256.get_out 1:/#.
   rewrite pack2wE 1:/#; have /= [-> ->] := divmod_mul 4 32 i j _ hj; 1: done; rewrite W4u32.bits32iE 1:// /#.
 qed.
@@ -2090,8 +2604,8 @@ hint simplify W128_bits64_bits32, W256_bits64_bits32, W256_bits128_bits32.
 (* Lemmas on \bits64                                                                 *)
 (* --------------------------------------------------------------------------------- *)
 
-lemma bits64_W16u8 ws i : 
-  W16u8.pack16_t ws \bits64 i = 
+lemma bits64_W16u8 ws i :
+  W16u8.pack16_t ws \bits64 i =
     if 0 <= i < 2 then W8u8.pack8 [ws.[8 * i]; ws.[8 * i + 1]; ws.[8 * i + 2]; ws.[8 * i + 3];
                                    ws.[8 * i + 4]; ws.[8 * i + 5]; ws.[8 * i + 6]; ws.[8 * i + 7]]
     else W64.zero.
@@ -2103,15 +2617,15 @@ proof.
   by move: hj; rewrite -(mema_iota 0 8) /= => -[|[|[|[|[|[|[|]]]]]]] ->.
 qed.
 
-lemma bits64_W16u8_red ws i : 
+lemma bits64_W16u8_red ws i :
   0 <= i < 2 =>
-  W16u8.pack16_t ws \bits64 i = 
+  W16u8.pack16_t ws \bits64 i =
     W8u8.pack8 [ws.[8 * i]; ws.[8 * i + 1]; ws.[8 * i + 2]; ws.[8 * i + 3];
                 ws.[8 * i + 4]; ws.[8 * i + 5]; ws.[8 * i + 6]; ws.[8 * i + 7]].
 proof. by move=> h;rewrite bits64_W16u8 h. qed.
 
-lemma bits64_W32u8 ws i : 
-  W32u8.pack32_t ws \bits64 i = 
+lemma bits64_W32u8 ws i :
+  W32u8.pack32_t ws \bits64 i =
     if 0 <= i < 4 then W8u8.pack8 [ws.[8 * i]; ws.[8 * i + 1]; ws.[8 * i + 2]; ws.[8 * i + 3];
                                    ws.[8 * i + 4]; ws.[8 * i + 5]; ws.[8 * i + 6]; ws.[8 * i + 7]]
     else W64.zero.
@@ -2123,17 +2637,17 @@ proof.
   by move: hj; rewrite -(mema_iota 0 8) /= => -[|[|[|[|[|[|[|]]]]]]] ->.
 qed.
 
-lemma bits64_W32u8_red ws i : 
+lemma bits64_W32u8_red ws i :
   0 <= i < 4 =>
-  W32u8.pack32_t ws \bits64 i = 
+  W32u8.pack32_t ws \bits64 i =
     W8u8.pack8 [ws.[8 * i]; ws.[8 * i + 1]; ws.[8 * i + 2]; ws.[8 * i + 3];
                 ws.[8 * i + 4]; ws.[8 * i + 5]; ws.[8 * i + 6]; ws.[8 * i + 7]].
 proof. by move=> h;rewrite bits64_W32u8 h. qed.
 
 hint simplify bits64_W16u8_red, bits64_W32u8_red.
 
-lemma bits64_W8u16 ws i : 
-  W8u16.pack8_t ws \bits64 i = 
+lemma bits64_W8u16 ws i :
+  W8u16.pack8_t ws \bits64 i =
     if 0 <= i < 2 then W4u16.pack4 [ws.[4 * i]; ws.[4 * i + 1]; ws.[4 * i + 2]; ws.[4 * i + 3] ] else W64.zero.
 proof.
   apply W4u16.wordP => j hj.
@@ -2143,14 +2657,14 @@ proof.
   by have [|[|[|]]]-> : j = 0 \/ j = 1 \/ j = 2 \/ j = 3 by smt().
 qed.
 
-lemma bits64_W8u16_red ws i : 
-  0 <= i < 2 => 
-  W8u16.pack8_t ws \bits64 i = 
+lemma bits64_W8u16_red ws i :
+  0 <= i < 2 =>
+  W8u16.pack8_t ws \bits64 i =
     W4u16.pack4 [ws.[4 * i]; ws.[4 * i + 1]; ws.[4 * i + 2]; ws.[4 * i + 3] ].
 proof. by move=> h;rewrite bits64_W8u16 h. qed.
 
-lemma bits64_W16u16 ws i : 
-  W16u16.pack16_t ws \bits64 i = 
+lemma bits64_W16u16 ws i :
+  W16u16.pack16_t ws \bits64 i =
     if 0 <= i < 4 then W4u16.pack4 [ws.[4 * i]; ws.[4 * i + 1]; ws.[4 * i + 2]; ws.[4 * i + 3] ] else W64.zero.
 proof.
   apply W4u16.wordP => j hj.
@@ -2160,16 +2674,16 @@ proof.
   by have [|[|[|]]]-> : j = 0 \/ j = 1 \/ j = 2 \/ j = 3 by smt().
 qed.
 
-lemma bits64_W16u16_red ws i : 
-  0 <= i < 4 => 
-  W16u16.pack16_t ws \bits64 i = 
+lemma bits64_W16u16_red ws i :
+  0 <= i < 4 =>
+  W16u16.pack16_t ws \bits64 i =
     W4u16.pack4 [ws.[4 * i]; ws.[4 * i + 1]; ws.[4 * i + 2]; ws.[4 * i + 3] ].
 proof. by move=> h;rewrite bits64_W16u16 h. qed.
 
 hint simplify bits64_W8u16_red, bits64_W16u16_red.
 
 lemma bits64_W4u32 ws i :
-  W4u32.pack4_t ws \bits64 i = 
+  W4u32.pack4_t ws \bits64 i =
     if 0 <= i < 2 then W2u32.pack2 [ws.[2 * i]; ws.[2 * i + 1]] else W64.zero.
 proof.
   apply W2u32.wordP => j hj.
@@ -2177,7 +2691,7 @@ proof.
   case: (0 <= i < 2) => hi; last by rewrite W2u32.get_zero W4u32.get_out 1:/#.
   rewrite /= W2u32.pack2bE 1:// /= W4u32.pack4bE 1:/#.
   by have [|]-> : j = 0 \/ j = 1 by smt().
-qed.  
+qed.
 
 lemma bits64_W4u32_red ws i :
   0 <= i < 2 =>
@@ -2185,7 +2699,7 @@ lemma bits64_W4u32_red ws i :
 proof. by move=> h;rewrite bits64_W4u32 h. qed.
 
 lemma bits64_W8u32 ws i :
-  W8u32.pack8_t ws \bits64 i = 
+  W8u32.pack8_t ws \bits64 i =
     if 0 <= i < 4 then W2u32.pack2 [ws.[2 * i]; ws.[2 * i + 1]] else W64.zero.
 proof.
   apply W2u32.wordP => j hj.
@@ -2193,24 +2707,24 @@ proof.
   case: (0 <= i < 4) => hi; last by rewrite W2u32.get_zero W8u32.get_out 1:/#.
   rewrite /= W2u32.pack2bE 1:// /= W8u32.pack8bE 1:/#.
   have [|]-> //= : j = 0 \/ j = 1 by smt().
-qed.  
+qed.
 
 lemma bits64_W8u32_red ws i :
-  0 <= i < 4 => 
+  0 <= i < 4 =>
   W8u32.pack8_t ws \bits64 i = W2u32.pack2 [ws.[2 * i]; ws.[2 * i + 1]].
 proof. by move=> h;rewrite bits64_W8u32 h. qed.
 
 hint simplify bits64_W4u32_red, bits64_W8u32_red.
 
-lemma bits64_W2u128 ws i : 
+lemma bits64_W2u128 ws i :
   W2u128.pack2_t ws \bits64 i = if 0 <= i < 4 then ws.[i%/2] \bits64 (i%%2) else W64.zero.
 proof.
-  apply W64.wordP => j hj; rewrite !bits64iE 1,2://. 
+  apply W64.wordP => j hj; rewrite !bits64iE 1,2://.
   case: (0 <= i < 4) => /= hi; last by rewrite W256.get_out 1:/#.
   rewrite pack2wE 1:/#; have /= [-> ->] := divmod_mul 2 64 i j _ hj; 1: done; rewrite W2u64.bits64iE 1:// /#.
 qed.
 
-lemma bits64_W2u128_red ws i : 
+lemma bits64_W2u128_red ws i :
   0 <= i < 4 => W2u128.pack2_t ws \bits64 i = ws.[i%/2] \bits64 (i%%2).
 proof. by move=> h;rewrite bits64_W2u128 h. qed.
 
@@ -2228,15 +2742,15 @@ hint simplify W256_bits128_bits64.
 (* Lemmas on \bits128                                                                *)
 (* --------------------------------------------------------------------------------- *)
 
-lemma bits128_W32u8 ws i : 
-  W32u8.pack32_t ws \bits128 i = 
+lemma bits128_W32u8 ws i :
+  W32u8.pack32_t ws \bits128 i =
    if  0 <= i < 2 then
     W16u8.pack16 [ws.[16 * i]; ws.[16 * i + 1]; ws.[16 * i + 2]; ws.[16 * i + 3];
                   ws.[16 * i + 4]; ws.[16 * i + 5]; ws.[16 * i + 6]; ws.[16 * i + 7];
                   ws.[16 * i + 8]; ws.[16 * i + 9]; ws.[16 * i + 10]; ws.[16 * i + 11];
                   ws.[16 * i + 12]; ws.[16 * i + 13]; ws.[16 * i + 14]; ws.[16 * i + 15]]
    else W128.zero.
-proof. 
+proof.
   apply W16u8.wordP => j hj.
   rewrite W256_bits128_bits8 1://.
   case: (0 <= i < 2) => hi; last by rewrite W16u8.get_zero W32u8.get_out 1:/#.
@@ -2244,22 +2758,22 @@ proof.
   by move: hj; rewrite -(mema_iota 0 16) /= => -[|[|[|[|[|[|[|[|[|[|[|[|[|[|[|]]]]]]]]]]]]]]] ->.
 qed.
 
-lemma bits128_W32u8_red ws i : 
+lemma bits128_W32u8_red ws i :
   0 <= i < 2 =>
-  W32u8.pack32_t ws \bits128 i = 
+  W32u8.pack32_t ws \bits128 i =
     W16u8.pack16 [ws.[16 * i]; ws.[16 * i + 1]; ws.[16 * i + 2]; ws.[16 * i + 3];
                   ws.[16 * i + 4]; ws.[16 * i + 5]; ws.[16 * i + 6]; ws.[16 * i + 7];
                   ws.[16 * i + 8]; ws.[16 * i + 9]; ws.[16 * i + 10]; ws.[16 * i + 11];
                   ws.[16 * i + 12]; ws.[16 * i + 13]; ws.[16 * i + 14]; ws.[16 * i + 15]].
 proof. by move=> hi;rewrite bits128_W32u8 hi. qed.
 
-lemma bits128_W16u16 ws i : 
-  W16u16.pack16_t ws \bits128 i = 
+lemma bits128_W16u16 ws i :
+  W16u16.pack16_t ws \bits128 i =
    if  0 <= i < 2 then
     W8u16.pack8 [ws.[8 * i]; ws.[8 * i + 1]; ws.[8 * i + 2]; ws.[8 * i + 3];
                  ws.[8 * i + 4]; ws.[8 * i + 5]; ws.[8 * i + 6]; ws.[8 * i + 7]]
    else W128.zero.
-proof. 
+proof.
   apply W8u16.wordP => j hj.
   rewrite W256_bits128_bits16 1://.
   case: (0 <= i < 2) => hi; last by rewrite W8u16.get_zero W16u16.get_out 1:/#.
@@ -2267,19 +2781,19 @@ proof.
   by move: hj; rewrite -(mema_iota 0 8) /= => -[|[|[|[|[|[|[|]]]]]]] ->.
 qed.
 
-lemma bits128_W16u16_red ws i : 
+lemma bits128_W16u16_red ws i :
   0 <= i < 2 =>
-  W16u16.pack16_t ws \bits128 i = 
+  W16u16.pack16_t ws \bits128 i =
     W8u16.pack8 [ws.[8 * i]; ws.[8 * i + 1]; ws.[8 * i + 2]; ws.[8 * i + 3];
                  ws.[8 * i + 4]; ws.[8 * i + 5]; ws.[8 * i + 6]; ws.[8 * i + 7]].
 proof. by move=> hi;rewrite bits128_W16u16 hi. qed.
 
-lemma bits128_W8u32 ws i : 
-  W8u32.pack8_t ws \bits128 i = 
+lemma bits128_W8u32 ws i :
+  W8u32.pack8_t ws \bits128 i =
    if  0 <= i < 2 then
     W4u32.pack4 [ws.[4 * i]; ws.[4 * i + 1]; ws.[4 * i + 2]; ws.[4 * i + 3]]
    else W128.zero.
-proof. 
+proof.
   apply W4u32.wordP => j hj.
   rewrite W256_bits128_bits32 1://.
   case: (0 <= i < 2) => hi; last by rewrite W4u32.get_zero W8u32.get_out 1:/#.
@@ -2287,26 +2801,26 @@ proof.
   by move: hj; rewrite -(mema_iota 0 4) /= => -[|[|[|]]] ->.
 qed.
 
-lemma bits128_W8u32_red ws i : 
-  0 <= i < 2 => 
-  W8u32.pack8_t ws \bits128 i = 
+lemma bits128_W8u32_red ws i :
+  0 <= i < 2 =>
+  W8u32.pack8_t ws \bits128 i =
     W4u32.pack4 [ws.[4 * i]; ws.[4 * i + 1]; ws.[4 * i + 2]; ws.[4 * i + 3]].
 proof. by move=> hi;rewrite bits128_W8u32 hi. qed.
 
-lemma bits128_W4u64 ws i : 
-  W4u64.pack4_t ws \bits128 i = 
+lemma bits128_W4u64 ws i :
+  W4u64.pack4_t ws \bits128 i =
    if  0 <= i < 2 then
     W2u64.pack2 [ws.[2 * i]; ws.[2* i + 1]]
    else W128.zero.
-proof. 
+proof.
   apply W2u64.wordP => j hj.
   rewrite W256_bits128_bits64 1://.
   case: (0 <= i < 2) => hi; last by rewrite W2u64.get_zero W4u64.get_out 1:/#.
-  rewrite /= W4u64.pack4bE 1:/# /= W2u64.pack2bE 1:// get_of_list 1://. 
+  rewrite /= W4u64.pack4bE 1:/# /= W2u64.pack2bE 1:// get_of_list 1://.
   by move: hj; rewrite -(mema_iota 0 2) /= => -[|] ->.
 qed.
 
-lemma bits128_W4u64_red ws i : 
+lemma bits128_W4u64_red ws i :
   0 <= i < 2 =>
   W4u64.pack4_t ws \bits128 i = W2u64.pack2 [ws.[2 * i]; ws.[2* i + 1]].
 proof. by move=> hi;rewrite bits128_W4u64 hi. qed.
@@ -2317,18 +2831,18 @@ hint simplify bits128_W32u8_red, bits128_W16u16_red, bits128_W8u32_red, bits128_
 (* Lemmas on pack                                                                    *)
 (* --------------------------------------------------------------------------------- *)
 
-lemma W2u16_W4u8 ws1 ws2 : 
+lemma W2u16_W4u8 ws1 ws2 :
   pack2 [W2u8.pack2_t ws1; W2u8.pack2_t ws2] = pack4 [ws1.[0]; ws1.[1]; ws2.[0]; ws2.[1]].
 proof. by apply W4u8.allP => /=. qed.
 
 lemma W4u16_W8u8 ws1 ws2 ws3 ws4 :
-  pack4 [W2u8.pack2_t ws1; W2u8.pack2_t ws2; W2u8.pack2_t ws3; W2u8.pack2_t ws4] = 
+  pack4 [W2u8.pack2_t ws1; W2u8.pack2_t ws2; W2u8.pack2_t ws3; W2u8.pack2_t ws4] =
   pack8 [ws1.[0]; ws1.[1]; ws2.[0]; ws2.[1]; ws3.[0]; ws3.[1]; ws4.[0]; ws4.[1]].
 proof. by apply W8u8.allP => /=. qed.
 
 lemma W8u16_W16u8 ws1 ws2 ws3 ws4 ws5 ws6 ws7 ws8:
   pack8 [W2u8.pack2_t ws1; W2u8.pack2_t ws2; W2u8.pack2_t ws3; W2u8.pack2_t ws4;
-         W2u8.pack2_t ws5; W2u8.pack2_t ws6; W2u8.pack2_t ws7; W2u8.pack2_t ws8 ] = 
+         W2u8.pack2_t ws5; W2u8.pack2_t ws6; W2u8.pack2_t ws7; W2u8.pack2_t ws8 ] =
   pack16 [ws1.[0]; ws1.[1]; ws2.[0]; ws2.[1]; ws3.[0]; ws3.[1]; ws4.[0]; ws4.[1];
          ws5.[0]; ws5.[1]; ws6.[0]; ws6.[1]; ws7.[0]; ws7.[1]; ws8.[0]; ws8.[1]].
 proof. by apply W16u8.allP => /=. qed.
@@ -2337,7 +2851,7 @@ lemma W16u16_W32u8 ws1 ws2 ws3 ws4 ws5 ws6 ws7 ws8 ws9 ws10 ws11 ws12 ws13 ws14 
   pack16 [W2u8.pack2_t ws1; W2u8.pack2_t ws2; W2u8.pack2_t ws3; W2u8.pack2_t ws4;
           W2u8.pack2_t ws5; W2u8.pack2_t ws6; W2u8.pack2_t ws7; W2u8.pack2_t ws8;
           W2u8.pack2_t ws9; W2u8.pack2_t ws10; W2u8.pack2_t ws11; W2u8.pack2_t ws12;
-          W2u8.pack2_t ws13; W2u8.pack2_t ws14; W2u8.pack2_t ws15; W2u8.pack2_t ws16] = 
+          W2u8.pack2_t ws13; W2u8.pack2_t ws14; W2u8.pack2_t ws15; W2u8.pack2_t ws16] =
   pack32 [ws1.[0]; ws1.[1]; ws2.[0]; ws2.[1]; ws3.[0]; ws3.[1]; ws4.[0]; ws4.[1];
           ws5.[0]; ws5.[1]; ws6.[0]; ws6.[1]; ws7.[0]; ws7.[1]; ws8.[0]; ws8.[1];
           ws9.[0]; ws9.[1]; ws10.[0]; ws10.[1]; ws11.[0]; ws11.[1]; ws12.[0]; ws12.[1];
@@ -2346,20 +2860,20 @@ proof. by apply W32u8.allP => /=. qed.
 
 hint simplify W2u16_W4u8, W4u16_W8u8, W8u16_W16u8, W16u16_W32u8.
 
-lemma W2u32_W8u8 ws1 ws2 : 
-  pack2 [W4u8.pack4_t ws1; W4u8.pack4_t ws2] = 
+lemma W2u32_W8u8 ws1 ws2 :
+  pack2 [W4u8.pack4_t ws1; W4u8.pack4_t ws2] =
   pack8 [ws1.[0]; ws1.[1]; ws1.[2]; ws1.[3]; ws2.[0]; ws2.[1]; ws2.[2]; ws2.[3]].
 proof. by apply W8u8.allP => /=. qed.
 
 lemma W4u32_W16u8 ws1 ws2 ws3 ws4 :
-  pack4 [W4u8.pack4_t ws1; W4u8.pack4_t ws2; W4u8.pack4_t ws3; W4u8.pack4_t ws4] = 
+  pack4 [W4u8.pack4_t ws1; W4u8.pack4_t ws2; W4u8.pack4_t ws3; W4u8.pack4_t ws4] =
   pack16 [ws1.[0]; ws1.[1]; ws1.[2]; ws1.[3]; ws2.[0]; ws2.[1]; ws2.[2]; ws2.[3];
           ws3.[0]; ws3.[1]; ws3.[2]; ws3.[3]; ws4.[0]; ws4.[1]; ws4.[2]; ws4.[3]].
 proof. by apply W16u8.allP => /=. qed.
 
 lemma W8u32_W32u8 ws1 ws2 ws3 ws4 ws5 ws6 ws7 ws8:
   pack8 [W4u8.pack4_t ws1; W4u8.pack4_t ws2; W4u8.pack4_t ws3; W4u8.pack4_t ws4;
-         W4u8.pack4_t ws5; W4u8.pack4_t ws6; W4u8.pack4_t ws7; W4u8.pack4_t ws8 ] = 
+         W4u8.pack4_t ws5; W4u8.pack4_t ws6; W4u8.pack4_t ws7; W4u8.pack4_t ws8 ] =
   pack32 [ws1.[0]; ws1.[1]; ws1.[2]; ws1.[3]; ws2.[0]; ws2.[1]; ws2.[2]; ws2.[3];
           ws3.[0]; ws3.[1]; ws3.[2]; ws3.[3]; ws4.[0]; ws4.[1]; ws4.[2]; ws4.[3];
           ws5.[0]; ws5.[1]; ws5.[2]; ws5.[3]; ws6.[0]; ws6.[1]; ws6.[2]; ws6.[3];
@@ -2369,13 +2883,13 @@ proof. by apply W32u8.allP => /=. qed.
 hint simplify W2u32_W8u8, W4u32_W16u8, W8u32_W32u8.
 
 lemma W2u64_W16u8 ws1 ws2:
-  pack2 [W8u8.pack8_t ws1; W8u8.pack8_t ws2] = 
+  pack2 [W8u8.pack8_t ws1; W8u8.pack8_t ws2] =
   pack16 [ws1.[0]; ws1.[1]; ws1.[2]; ws1.[3]; ws1.[4]; ws1.[5]; ws1.[6]; ws1.[7];
           ws2.[0]; ws2.[1]; ws2.[2]; ws2.[3]; ws2.[4]; ws2.[5]; ws2.[6]; ws2.[7]].
 proof. by apply W16u8.allP => /=. qed.
 
 lemma W4u64_W32u8 ws1 ws2 ws3 ws4:
-  pack4 [W8u8.pack8_t ws1; W8u8.pack8_t ws2; W8u8.pack8_t ws3; W8u8.pack8_t ws4] = 
+  pack4 [W8u8.pack8_t ws1; W8u8.pack8_t ws2; W8u8.pack8_t ws3; W8u8.pack8_t ws4] =
   pack32 [ws1.[0]; ws1.[1]; ws1.[2]; ws1.[3]; ws1.[4]; ws1.[5]; ws1.[6]; ws1.[7];
           ws2.[0]; ws2.[1]; ws2.[2]; ws2.[3]; ws2.[4]; ws2.[5]; ws2.[6]; ws2.[7];
           ws3.[0]; ws3.[1]; ws3.[2]; ws3.[3]; ws3.[4]; ws3.[5]; ws3.[6]; ws3.[7];
@@ -2385,7 +2899,7 @@ proof. by apply W32u8.allP => /=. qed.
 hint simplify W2u64_W16u8, W4u64_W32u8.
 
 lemma W2u128_W32u8 ws1 ws2:
-  pack2 [W16u8.pack16_t ws1; W16u8.pack16_t ws2] = 
+  pack2 [W16u8.pack16_t ws1; W16u8.pack16_t ws2] =
   pack32 [ws1.[0]; ws1.[1]; ws1.[2]; ws1.[3]; ws1.[4]; ws1.[5]; ws1.[6]; ws1.[7];
           ws1.[8]; ws1.[9]; ws1.[10]; ws1.[11]; ws1.[12]; ws1.[13]; ws1.[14]; ws1.[15];
           ws2.[0]; ws2.[1]; ws2.[2]; ws2.[3]; ws2.[4]; ws2.[5]; ws2.[6]; ws2.[7];
@@ -2394,18 +2908,18 @@ proof. by apply W32u8.allP => /=. qed.
 
 hint simplify W2u128_W32u8.
 
-lemma W2u32_W4u16 ws1 ws2 : 
+lemma W2u32_W4u16 ws1 ws2 :
   pack2 [W2u16.pack2_t ws1; W2u16.pack2_t ws2] = pack4 [ws1.[0]; ws1.[1]; ws2.[0]; ws2.[1]].
 proof. by apply W4u16.allP => /=. qed.
 
 lemma W4u32_W8u16 ws1 ws2 ws3 ws4 :
-  pack4 [W2u16.pack2_t ws1; W2u16.pack2_t ws2; W2u16.pack2_t ws3; W2u16.pack2_t ws4] = 
+  pack4 [W2u16.pack2_t ws1; W2u16.pack2_t ws2; W2u16.pack2_t ws3; W2u16.pack2_t ws4] =
   pack8 [ws1.[0]; ws1.[1]; ws2.[0]; ws2.[1]; ws3.[0]; ws3.[1]; ws4.[0]; ws4.[1]].
 proof. by apply W8u16.allP => /=. qed.
 
 lemma W8u32_W16u16 ws1 ws2 ws3 ws4 ws5 ws6 ws7 ws8:
   pack8 [W2u16.pack2_t ws1; W2u16.pack2_t ws2; W2u16.pack2_t ws3; W2u16.pack2_t ws4;
-         W2u16.pack2_t ws5; W2u16.pack2_t ws6; W2u16.pack2_t ws7; W2u16.pack2_t ws8 ] = 
+         W2u16.pack2_t ws5; W2u16.pack2_t ws6; W2u16.pack2_t ws7; W2u16.pack2_t ws8 ] =
   pack16 [ws1.[0]; ws1.[1]; ws2.[0]; ws2.[1]; ws3.[0]; ws3.[1]; ws4.[0]; ws4.[1];
          ws5.[0]; ws5.[1]; ws6.[0]; ws6.[1]; ws7.[0]; ws7.[1]; ws8.[0]; ws8.[1]].
 proof. by apply W16u16.allP => /=. qed.
@@ -2413,13 +2927,13 @@ proof. by apply W16u16.allP => /=. qed.
 hint simplify W2u32_W4u16, W4u32_W8u16, W8u32_W16u16.
 
 lemma W2u64_W8u16 ws1 ws2:
-  pack2 [W4u16.pack4_t ws1; W4u16.pack4_t ws2] = 
+  pack2 [W4u16.pack4_t ws1; W4u16.pack4_t ws2] =
   pack8 [ws1.[0]; ws1.[1]; ws1.[2]; ws1.[3];
          ws2.[0]; ws2.[1]; ws2.[2]; ws2.[3]].
 proof. by apply W8u16.allP => /=. qed.
 
 lemma W4u64_W16u16 ws1 ws2 ws3 ws4:
-  pack4 [W4u16.pack4_t ws1; W4u16.pack4_t ws2; W4u16.pack4_t ws3; W4u16.pack4_t ws4] = 
+  pack4 [W4u16.pack4_t ws1; W4u16.pack4_t ws2; W4u16.pack4_t ws3; W4u16.pack4_t ws4] =
   pack16 [ws1.[0]; ws1.[1]; ws1.[2]; ws1.[3]; ws2.[0]; ws2.[1]; ws2.[2]; ws2.[3];
           ws3.[0]; ws3.[1]; ws3.[2]; ws3.[3]; ws4.[0]; ws4.[1]; ws4.[2]; ws4.[3]].
 proof. by apply W16u16.allP => /=. qed.
@@ -2431,12 +2945,12 @@ lemma W2u64_W4u32 ws1 ws2:
 proof. by apply W4u32.allP => /=. qed.
 
 lemma W4u64_W8u32 ws1 ws2 ws3 ws4 :
-  pack4 [W2u32.pack2_t ws1; W2u32.pack2_t ws2; W2u32.pack2_t ws3; W2u32.pack2_t ws4] = 
+  pack4 [W2u32.pack2_t ws1; W2u32.pack2_t ws2; W2u32.pack2_t ws3; W2u32.pack2_t ws4] =
   pack8 [ws1.[0]; ws1.[1]; ws2.[0]; ws2.[1]; ws3.[0]; ws3.[1]; ws4.[0]; ws4.[1]].
 proof. by apply W8u32.allP => /=. qed.
 
 lemma W2u128_W8u32 ws1 ws2 :
-  pack2 [W4u32.pack4_t ws1; W4u32.pack4_t ws2] = 
+  pack2 [W4u32.pack4_t ws1; W4u32.pack4_t ws2] =
   pack8 [ws1.[0]; ws1.[1]; ws1.[2]; ws1.[3]; ws2.[0]; ws2.[1]; ws2.[2]; ws2.[3]].
 proof. by apply W8u32.allP => /=. qed.
 
@@ -2447,9 +2961,3 @@ lemma W2u128_W4u64 ws1 ws2:
 proof. by apply W4u64.allP => /=. qed.
 
 hint simplify W2u128_W4u64.
-
-
-
-
-
-
