eclib/JMemory.ec
@@ -13,20 +13,20 @@ export W8List.
 type address = int.
 
 type global_mem_t.
-  
+
 op "_.[_]" : global_mem_t -> address -> W8.t.
 op "_.[_<-_]" : global_mem_t -> address -> W8.t -> global_mem_t.
 
 axiom mem_eq_ext (m1 m2:global_mem_t) : (forall j, m1.[j] = m2.[j]) => m1 = m2.
 
-axiom get_setE m x y w : 
+axiom get_setE m x y w :
   m.[x <- w].[y] = if y = x then w else m.[y].
 
-lemma get_set_eqE_s m x y w : 
+lemma get_set_eqE_s m x y w :
   y = x => m.[x <- w].[y] = w.
 proof. by rewrite get_setE => ->. qed.
 
-lemma get_set_neqE_s m x y w : 
+lemma get_set_neqE_s m x y w :
   y <> x => m.[x <- w].[y] = m.[y].
 proof. by rewrite get_setE => ->. qed.
 
@@ -41,7 +41,7 @@ axiom allocated8_setE y w m x: allocated8 m.[y<-w] x = allocated8 m x.
 op stores (m : global_mem_t) (a : address) (w : W8.t list) =
   foldl (fun (m:global_mem_t) i => m.[a + i <- w.[i]]) m (iota_ 0 (size w)).
 
-lemma foldl_in_eq (f1 f2:'a -> 'b -> 'a) (s:'b list) a : 
+lemma foldl_in_eq (f1 f2:'a -> 'b -> 'a) (s:'b list) a :
    (forall a b, b \in s => f1 a b = f2 a b) => foldl f1 a s = foldl f2 a s.
 proof.
   elim: s a => [ | b s hrec] a //= hin.
@@ -53,7 +53,7 @@ proof.
   rewrite /stores /= iota_add 1:// 1:List.size_ge0.
   rewrite foldl_cat (addzC 0 1) iota_addl /=.
   rewrite -(revK (iota_ 0 (size ws))) map_rev !foldl_rev foldr_map /=.
-  rewrite -!foldl_rev !revK;apply foldl_in_eq => m0 i /mem_iota /= h /#. 
+  rewrite -!foldl_rev !revK;apply foldl_in_eq => m0 i /mem_iota /= h /#.
 qed.
 
 lemma allocated8_stores ws a m x : allocated8 (stores m a ws) x = allocated8 m x.
@@ -68,23 +68,23 @@ proof.
   + by rewrite /stores /= /#.
   rewrite stores_cons hrec /= get_setE.  smt (size_ge0).
 qed.
-  
+
 (* ------------------------------------------------------------------- *)
 op loadW8   (m : global_mem_t) (a : address) = m.[a].
 
-op loadW16  (m : global_mem_t) (a : address) = 
+op loadW16  (m : global_mem_t) (a : address) =
   pack2_t (W2u8.Pack.init (fun i => m.[a + i])).
 
-op loadW32  (m : global_mem_t) (a : address) = 
+op loadW32  (m : global_mem_t) (a : address) =
   pack4_t (W4u8.Pack.init (fun i => m.[a + i])).
 
-op loadW64  (m : global_mem_t) (a : address) = 
+op loadW64  (m : global_mem_t) (a : address) =
   pack8_t (W8u8.Pack.init (fun i => m.[a + i])).
 
-op loadW128 (m : global_mem_t) (a : address) = 
+op loadW128 (m : global_mem_t) (a : address) =
   pack16_t (W16u8.Pack.init (fun i => m.[a + i])).
 
-op loadW256 (m : global_mem_t) (a : address) = 
+op loadW256 (m : global_mem_t) (a : address) =
   pack32_t (W32u8.Pack.init (fun i => m.[a + i])).
 
 lemma loadW32_bits8 m p i : 0 <= i < 4 =>
@@ -97,17 +97,29 @@ proof. by move=> hi;rewrite /loadW128 pack16bE // initiE. qed.
 
 lemma loadW128_bits32 m p i : 0 <= i < 4 =>
   loadW128 m p \bits32 i = loadW32 m (p + i * 4).
-proof. 
+proof.
   move=> hi; rewrite /loadW128 /loadW32.
   apply W32.wordP => j hj.
   rewrite bits32iE // pack4wE // initiE; 1:by apply divz_cmp.
-  rewrite pack16wE; 1:by apply W4u32.in_bound. 
+  rewrite pack16wE; 1:by apply W4u32.in_bound.
   rewrite initiE /=; 1:by apply divz_cmp => //=;apply W4u32.in_bound.
-  have -> : i * 32 = (i * 4) * 8 by ring. 
-  by rewrite modzMDl divzMDl // -addzA. 
+  have -> : i * 32 = (i * 4) * 8 by ring.
+  by rewrite modzMDl divzMDl // -addzA.
 qed.
 
-lemma load4u8 mem p : 
+lemma loadW128_bits64 m p i : 0 <= i < 2 =>
+  loadW128 m p \bits64 i = loadW64 m (p + i * 8).
+proof.
+  move=> hi; rewrite /loadW128 /loadW64.
+  apply W64.wordP => j hj.
+  rewrite bits64iE // pack8wE // initiE; 1:by apply divz_cmp.
+  rewrite pack16wE; 1:by apply W2u64.in_bound.
+  rewrite initiE /=; 1:by apply divz_cmp => //=;apply W2u64.in_bound.
+  have -> : i * 64 = (i * 8) * 8 by ring.
+  by rewrite modzMDl divzMDl // -addzA.
+qed.
+
+lemma load4u8 mem p :
   pack4
     [loadW8 mem p;
      loadW8 mem (p + 1);
@@ -124,7 +136,7 @@ proof.
   by rewrite pack4K initiE.
 qed.
 
-lemma load4u32 mem p : 
+lemma load4u32 mem p :
   pack4
     [loadW32 mem p;
      loadW32 mem (p + 4);
@@ -139,6 +151,18 @@ proof.
   + by apply W4u32.Pack.all_eqP; rewrite /all_eq.
   apply (can_inj _ _ W4u32.unpack32K); apply W4u32.Pack.packP => i hi.
   by rewrite pack4K initiE //=  get_unpack32 // loadW128_bits32.
+qed.
+
+lemma load2u64 mem p:
+   pack2 [loadW64 mem p; loadW64 mem (p + 8)]
+   = loadW128 mem p.
+proof.
+  have ->: W2u64.Pack.of_list
+         [loadW64 mem p; loadW64 mem (p + 8)] =
+         W2u64.Pack.init (fun i => loadW64 mem (p + i * 8)).
+  + by apply W2u64.Pack.all_eqP; rewrite /all_eq.
+  apply (can_inj _ _ W2u64.unpack64K); apply W2u64.Pack.packP => i hi.
+  by rewrite pack2K initiE //=  get_unpack64 // loadW128_bits64.
 qed.
 
 (* ------------------------------------------------------------------- *)
@@ -166,7 +190,7 @@ op storeW256 (m : global_mem_t) (a : address) (w : W256.t) =
   stores m a (to_list (unpack8 w))
 axiomatized by storeW256E.
 
-lemma pack4u32_bits8_nth i (ws:W32.t list) : 0 <= i < 16 => 
+lemma pack4u32_bits8_nth i (ws:W32.t list) : 0 <= i < 16 =>
   W4u32.pack4 ws \bits8 i = nth W32.zero ws (i %/ 4) \bits8 (i%%4).
 proof.
   move=> hi; rewrite -W4u32.Pack.get_of_list; first by apply divz_cmp.
@@ -177,13 +201,24 @@ proof.
   congr; rewrite {1}(divz_eq i 4); ring.
 qed.
 
-lemma store4u32 mem ptr w0 w1 w2 w3 : 
+lemma pack2u64_bits8_nth i (ws:W64.t list) : 0 <= i < 16 =>
+  W2u64.pack2 ws \bits8 i = nth W64.zero ws (i %/ 8) \bits8 (i%%8).
+proof.
+  move=> hi; rewrite -W2u64.Pack.get_of_list; first by apply divz_cmp.
+  move: (W2u64.Pack.of_list ws) => w.
+  apply W8.wordP => k hk.
+  rewrite -W2u64.pack2bE; 1: by apply divz_cmp.
+  rewrite bits8iE // bits8iE // bits64iE; 1: smt(modz_cmp).
+  congr; rewrite {1}(divz_eq i 8); ring.
+qed.
+
+lemma store4u32 mem ptr w0 w1 w2 w3 :
   storeW128 mem ptr (W4u32.pack4 [w0; w1; w2; w3]) =
-  storeW32 
-    (storeW32 
-       (storeW32 
-          (storeW32 mem ptr w0) 
-          (ptr + 4) w1) 
+  storeW32
+    (storeW32
+       (storeW32
+          (storeW32 mem ptr w0)
+          (ptr + 4) w1)
        (ptr + 8) w2)
     (ptr + 12) w3.
 proof.
@@ -191,13 +226,21 @@ proof.
   by rewrite /W4u8.Pack.to_list /mkseq /= /stores.
 qed.
 
+lemma store2u64 mem ptr w0 w1:
+  storeW128 mem ptr (W2u64.pack2 [w0; w1]) =
+  storeW64 (storeW64 mem ptr w0) (ptr + 8) w1.
+proof.
+  rewrite storeW128E !storeW64E.
+  by rewrite /W2u16.Pack.to_list /mkseq /= /stores /=.
+qed.
+
 lemma store4u8 mem ptr w0 w1 w2 w3 :
   storeW32 mem ptr (W4u8.pack4 [w0; w1; w2; w3]) =
-  storeW8 
-    (storeW8 
-       (storeW8 
-          (storeW8 mem ptr w0) 
-          (ptr + 1) w1) 
+  storeW8
+    (storeW8
+       (storeW8
+          (storeW8 mem ptr w0)
+          (ptr + 1) w1)
        (ptr + 2) w2)
     (ptr + 3) w3.
 proof. by rewrite storeW32E !storeW8E. qed.
@@ -216,13 +259,13 @@ module Glob = {
 (* ------------------------------------------------------------------- *)
 (* Safety                                                              *)
 
-op is_align (ws:wsize) (a:address) = 
+op is_align (ws:wsize) (a:address) =
   wsize_i ws %| a.
 
-op allocated (m:global_mem_t) (p:address) (N:int) : bool = 
+op allocated (m:global_mem_t) (p:address) (N:int) : bool =
   forall i, 0 <= i < N => allocated8 m (p + i).
 
-op is_valid (m:global_mem_t) (a:address) (ws:wsize) = 
+op is_valid (m:global_mem_t) (a:address) (ws:wsize) =
   allocated m a (wsize_i ws) /\ is_align ws a
 axiomatized by is_validE.
 
@@ -231,13 +274,13 @@ op valid_range (w:wsize) (mem:global_mem_t) (ptr:address) (len:int) =
 
 (* ------------------------------------------------------------------- *)
 
-lemma is_align_le w2 w1 ptr: 
+lemma is_align_le w2 w1 ptr:
   wsize_i w1 <= wsize_i w2 => is_align w2 ptr => is_align w1 ptr.
 proof.
   by rewrite /is_align => hw; apply dvdz_trans; apply div_le_wsize.
 qed.
 
-lemma is_align_add w ptr ofs: 
+lemma is_align_add w ptr ofs:
   wsize_i w %| ofs => is_align w ptr => is_align w (ptr + ofs).
 proof.
   by rewrite /is_align => h1 h2; apply dvdzD.
@@ -252,7 +295,7 @@ proof.
   by rewrite allocated8_stores h.
 qed.
 
-lemma allocate_le m p (N1 N2:int) : 
+lemma allocate_le m p (N1 N2:int) :
   N1 <= N2 =>
   allocated m p N2 => allocated m p N1.
 proof. rewrite /allocated => hle h i hi;apply h => /#. qed.
@@ -260,28 +303,28 @@ proof. rewrite /allocated => hle h i hi;apply h => /#. qed.
 (* ------------------------------------------------------------------- *)
 
 lemma valid_range_le (len1 len2:int) w mem ptr  :
-  len1 <= len2 =>   
+  len1 <= len2 =>
   valid_range w mem ptr len2 =>
   valid_range w mem ptr len1.
 proof. by move=> hle hv i hlt; apply hv => /#. qed.
 
-lemma is_valid_valid_range w1 w2 mem ptr : 
-  wsize_i w1 <= wsize_i w2 => 
+lemma is_valid_valid_range w1 w2 mem ptr :
+  wsize_i w1 <= wsize_i w2 =>
   is_valid mem ptr w2 =>
   valid_range w1 mem ptr (wsize_i w2 %/ wsize_i w1).
 proof.
   rewrite /valid_range is_validE => hw [ha hia] i hi.
   rewrite is_validE is_align_add /=.
-  + by apply modzMr. 
+  + by apply modzMr.
   + by apply: is_align_le hia.
   move=> k hk /=;rewrite -addzA;apply ha;split;[smt (gt0_wsize_i)|move=> ?].
   apply: (ltr_le_trans ((i + 1) * wsize_i w1)); 1: smt ().
-  rewrite (divz_eq (wsize_i w2) (wsize_i w1)). 
+  rewrite (divz_eq (wsize_i w2) (wsize_i w1)).
   smt (modz_cmp gt0_wsize_i).
 qed.
 
-lemma valid_range_size_le w1 w2 mem ptr len : 
-   wsize_i w1 <= wsize_i w2 => 
+lemma valid_range_size_le w1 w2 mem ptr len :
+   wsize_i w1 <= wsize_i w2 =>
    valid_range w2 mem ptr len =>
    valid_range w1 mem ptr (len * (wsize_i w2 %/ wsize_i w1)).
 proof.
@@ -290,11 +333,11 @@ proof.
   have gt0_dw : 0 < dw.
   + by apply ltz_divRL => //; apply div_le_wsize.
   have := hv (i %/ dw) _.
-  + apply divz_cmp => //. 
+  + apply divz_cmp => //.
   move=> /(is_valid_valid_range _ _ _ _ hw) /(_ (i %% dw) _) /=.
-  + by apply modz_cmp.  
+  + by apply modz_cmp.
   have <- := divzK _ _ (div_le_wsize _ _ hw); rewrite -/dw.
-  have -> : ptr + dw * wsize_i w1 * (i %/ dw) + wsize_i w1 * (i %% dw) = 
+  have -> : ptr + dw * wsize_i w1 * (i %/ dw) + wsize_i w1 * (i %% dw) =
             ptr + wsize_i w1 * ((i %/ dw) * dw + i %% dw) by ring.
   by rewrite -divz_eq.
 qed.
@@ -313,15 +356,15 @@ proof.
   move=> i hi.
   have := hr (i %/ wsize_i w1) _.
   + split; 1: by apply divz_ge0;[ apply gt0_wsize_i | case hi].
-    move=> ?;apply ltz_divRL => //; 1: by apply div_le_wsize. 
+    move=> ?;apply ltz_divRL => //; 1: by apply div_le_wsize.
     by have := divz_eq i (wsize_i w1); have := modz_cmp i (wsize_i w1) _ => // /#.
   rewrite is_validE; move => [] /(_ (i%%wsize_i w1) _); 1: by apply modz_cmp.
   by rewrite mulzC -addzA -divz_eq.
 qed.
-  
+
 lemma valid_range_size_ge w1 w2 mem ptr len1 len2 :
-  is_align w2 ptr => 
-  wsize_i w1 <= wsize_i w2 =>  
+  is_align w2 ptr =>
+  wsize_i w1 <= wsize_i w2 =>
   (wsize_i w2 %/ wsize_i w1) * len2 <= len1 =>
   valid_range w1 mem ptr len1 =>
   valid_range w2 mem ptr len2.
@@ -334,20 +377,20 @@ proof.
   have gt0_dw : 0 < wsize_i w2 %/ wsize_i w1.
   + by apply ltz_divRL => //; apply div_le_wsize.
   have := hv ((wsize_i w2 %/ wsize_i w1) * i + k) _.
-  + split. smt(). 
+  + split. smt().
     move=> ?;apply (ltr_le_trans (wsize_i w2 %/ wsize_i w1 * (i + 1))).
-    + smt(). 
+    + smt().
     by apply ler_wpmul2l;[apply ltzW | smt()].
   rewrite Ring.IntID.mulrDr -mulzA (mulzC(wsize_i w1)) divzK ?addzA //.
   by apply div_le_wsize.
 qed.
 
 lemma valid_range_add (k:int) w mem ptr len :
-  0 <= k <= len =>   
+  0 <= k <= len =>
   valid_range w mem ptr len =>
   valid_range w mem (ptr + k * wsize_i w) (len - k).
 proof.
-  move=> hk hv i hi /=. 
+  move=> hk hv i hi /=.
   have -> : ptr + k * wsize_i w + wsize_i w * i = ptr + wsize_i w * (k + i) by ring.
   apply hv => /#.
 qed.
@@ -364,8 +407,8 @@ proof.
 qed.
 
 (* ------------------------------------------------------------------- *)
-    
-lemma is_valid_store8 mem sz ptr1 ptr2 w : 
+
+lemma is_valid_store8 mem sz ptr1 ptr2 w :
   is_valid (storeW8 mem ptr2 w) ptr1 sz = is_valid mem ptr1 sz.
 proof.
   rewrite !is_validE storeW8E /allocated;congr.
@@ -375,37 +418,37 @@ proof.
 qed.
 hint simplify is_valid_store8.
 
-lemma is_valid_store16 mem sz ptr1 ptr2 w : 
+lemma is_valid_store16 mem sz ptr1 ptr2 w :
   is_valid (storeW16 mem ptr2 w) ptr1 sz = is_valid mem ptr1 sz.
 proof.
- by rewrite !is_validE storeW16E allocated_stores. 
+ by rewrite !is_validE storeW16E allocated_stores.
 qed.
 hint simplify is_valid_store16.
 
-lemma is_valid_store32 mem sz ptr1 ptr2 w : 
+lemma is_valid_store32 mem sz ptr1 ptr2 w :
   is_valid (storeW32 mem ptr2 w) ptr1 sz = is_valid mem ptr1 sz.
 proof.
- by rewrite !is_validE storeW32E allocated_stores. 
+ by rewrite !is_validE storeW32E allocated_stores.
 qed.
 hint simplify is_valid_store32.
 
-lemma is_valid_store64 mem sz ptr1 ptr2 w : 
+lemma is_valid_store64 mem sz ptr1 ptr2 w :
   is_valid (storeW64 mem ptr2 w) ptr1 sz = is_valid mem ptr1 sz.
 proof.
- by rewrite !is_validE storeW64E allocated_stores. 
+ by rewrite !is_validE storeW64E allocated_stores.
 qed.
 hint simplify is_valid_store64.
 
-lemma is_valid_store128 mem sz ptr1 ptr2 w : 
+lemma is_valid_store128 mem sz ptr1 ptr2 w :
   is_valid (storeW128 mem ptr2 w) ptr1 sz = is_valid mem ptr1 sz.
 proof.
- by rewrite !is_validE storeW128E allocated_stores. 
+ by rewrite !is_validE storeW128E allocated_stores.
 qed.
 hint simplify is_valid_store128.
 
-lemma is_valid_store256 mem sz ptr1 ptr2 w : 
+lemma is_valid_store256 mem sz ptr1 ptr2 w :
   is_valid (storeW256 mem ptr2 w) ptr1 sz = is_valid mem ptr1 sz.
 proof.
- by rewrite !is_validE storeW256E allocated_stores. 
+ by rewrite !is_validE storeW256E allocated_stores.
 qed.
 hint simplify is_valid_store256.
