eclib/JWord_array.ec
@@ -9,7 +9,7 @@ abstract theory WArray.
     type elem <- W8.t,
     op dfl    <- W8.zero.
 
-  op get8 (t:t) (i:int)  : W8.t = t.[i]. 
+  op get8 (t:t) (i:int)  : W8.t = t.[i].
 
   op get16 (t:t) (i:int) : W16.t =
     pack2_t (W2u8.Pack.init (fun j => t.[2*i + j]))
@@ -31,47 +31,47 @@ abstract theory WArray.
     pack32_t (W32u8.Pack.init (fun j => t.[32*i + j]))
   axiomatized by get256E.
 
-  op set8 (t:t) (i:int) (w:W8.t) : t = t.[i <- w]. 
+  op set8 (t:t) (i:int) (w:W8.t) : t = t.[i <- w].
 
-  op set16 (t:t) (i:int) (w:W16.t) = 
+  op set16 (t:t) (i:int) (w:W16.t) =
     init (fun k => if 2*i <= k < 2*(i+1) then w \bits8 (k - 2*i) else t.[k])
   axiomatized by set16E.
 
-  op set32 (t:t) (i:int) (w:W32.t) = 
+  op set32 (t:t) (i:int) (w:W32.t) =
     init (fun k => if 4*i <= k < 4*(i+1) then w \bits8 (k - 4*i) else t.[k])
   axiomatized by set32E.
 
-  op set64 (t:t) (i:int) (w:W64.t) = 
+  op set64 (t:t) (i:int) (w:W64.t) =
     init (fun k => if 8*i <= k < 8*(i+1) then w \bits8 (k - 8*i) else t.[k])
   axiomatized by set64E.
 
-  op set128 (t:t) (i:int) (w:W128.t) = 
+  op set128 (t:t) (i:int) (w:W128.t) =
     init (fun k => if 16*i <= k < 16*(i+1) then w \bits8 (k - 16*i) else t.[k])
   axiomatized by set128E.
 
-  op set256 (t:t) (i:int) (w:W256.t) = 
+  op set256 (t:t) (i:int) (w:W256.t) =
     init (fun k => if 32*i <= k < 32*(i+1) then w \bits8 (k - 32*i) else t.[k])
   axiomatized by set256E.
 
   (* ----------------------------------------------------- *)
 
-  lemma get_set8E t x y w: 
+  lemma get_set8E t x y w:
     0 <= x < size =>
     get8 (set8 t x w) y = if y = x then w else get8 t y.
   proof. apply get_setE. qed.
 
-  lemma get8_set16E t x y w : 
+  lemma get8_set16E t x y w :
     0 <= x => 2*(x + 1) <= WArray.size =>
     get8 (set16 t x w) y = if 2*x <= y < 2*(x+1) then w \bits8 (y - 2*x) else get8 t y.
   proof.
     move=> hx hs; rewrite set16E /get8.
     case: (2 * x <= y < 2 * (x + 1)) => hy.
-    + by rewrite initiE 1:/# /= hy. 
+    + by rewrite initiE 1:/# /= hy.
     case: (0 <= y < WArray.size) => hy1; last by rewrite !get_out.
     rewrite initiE //= /#.
   qed.
 
-  lemma get_set16E t x y w: 
+  lemma get_set16E t x y w:
     0 <= x => 2*(x + 1) <= WArray.size =>
     get16 (set16 t x w) y = if y = x then w else get16 t y.
   proof.
@@ -83,18 +83,18 @@ abstract theory WArray.
     by case: (0 <= 2 * y + k < WArray.size) => [ /# | /get_out ->].
   qed.
 
-  lemma get8_set32E t x y w : 
+  lemma get8_set32E t x y w :
     0 <= x => 4*(x + 1) <= WArray.size =>
     get8 (set32 t x w) y = if 4*x <= y < 4*(x+1) then w \bits8 (y - 4*x) else get8 t y.
   proof.
     move=> hx hs; rewrite set32E /get8.
     case: (4 * x <= y < 4 * (x + 1)) => hy.
-    + by rewrite initiE 1:/# /= hy. 
+    + by rewrite initiE 1:/# /= hy.
     case: (0 <= y < WArray.size) => hy1; last by rewrite !get_out.
     rewrite initiE //= /#.
   qed.
 
-  lemma get_set32E t x y w: 
+  lemma get_set32E t x y w:
     0 <= x => 4*(x + 1) <= WArray.size =>
     get32 (set32 t x w) y = if y = x then w else get32 t y.
   proof.
@@ -106,18 +106,18 @@ abstract theory WArray.
     by case: (0 <= 4 * y + k < WArray.size) => [ /# | /get_out ->].
   qed.
 
-  lemma get8_set64E t x y w : 
+  lemma get8_set64E t x y w :
     0 <= x => 8*(x + 1) <= WArray.size =>
     get8 (set64 t x w) y = if 8*x <= y < 8*(x+1) then w \bits8 (y - 8*x) else get8 t y.
   proof.
     move=> hx hs; rewrite set64E /get8.
     case: (8 * x <= y < 8 * (x + 1)) => hy.
-    + by rewrite initiE 1:/# /= hy. 
+    + by rewrite initiE 1:/# /= hy.
     case: (0 <= y < WArray.size) => hy1; last by rewrite !get_out.
     rewrite initiE //= /#.
   qed.
 
-  lemma get_set64E t x y w: 
+  lemma get_set64E t x y w:
     0 <= x => 8*(x + 1) <= WArray.size =>
     get64 (set64 t x w) y = if y = x then w else get64 t y.
   proof.
@@ -129,18 +129,18 @@ abstract theory WArray.
     by case: (0 <= 8 * y + k < WArray.size) => [ /# | /get_out ->].
   qed.
 
-  lemma get8_set128E t x y w : 
+  lemma get8_set128E t x y w :
     0 <= x => 16*(x + 1) <= WArray.size =>
     get8 (set128 t x w) y = if 16*x <= y < 16*(x+1) then w \bits8 (y - 16*x) else get8 t y.
   proof.
     move=> hx hs; rewrite set128E /get8.
     case: (16 * x <= y < 16 * (x + 1)) => hy.
-    + by rewrite initiE 1:/# /= hy. 
+    + by rewrite initiE 1:/# /= hy.
     case: (0 <= y < WArray.size) => hy1; last by rewrite !get_out.
     rewrite initiE //= /#.
   qed.
 
-  lemma get_set128E t x y w: 
+  lemma get_set128E t x y w:
     0 <= x => 16*(x + 1) <= WArray.size =>
     get128 (set128 t x w) y = if y = x then w else get128 t y.
   proof.
@@ -152,18 +152,18 @@ abstract theory WArray.
     by case: (0 <= 16 * y + k < WArray.size) => [ /# | /get_out ->].
   qed.
 
-  lemma get8_set256E t x y w : 
+  lemma get8_set256E t x y w :
     0 <= x => 32*(x + 1) <= WArray.size =>
     get8 (set256 t x w) y = if 32*x <= y < 32*(x+1) then w \bits8 (y - 32*x) else get8 t y.
   proof.
     move=> hx hs; rewrite set256E /get8.
     case: (32 * x <= y < 32 * (x + 1)) => hy.
-    + by rewrite initiE 1:/# /= hy. 
+    + by rewrite initiE 1:/# /= hy.
     case: (0 <= y < WArray.size) => hy1; last by rewrite !get_out.
     rewrite initiE //= /#.
   qed.
 
-  lemma get_set256E t x y w: 
+  lemma get_set256E t x y w:
     0 <= x => 32*(x + 1) <= WArray.size =>
     get256 (set256 t x w) y = if y = x then w else get256 t y.
   proof.
@@ -183,23 +183,23 @@ abstract theory WArray.
 
   (* ------------------------------------------------- *)
 
-  op init8 (f:int -> W8.t) = 
+  op init8 (f:int -> W8.t) =
     init f.
 
   op init16 (f:int -> W16.t) =
     init (fun i => f (i %/ 2) \bits8 (i%%2)).
 
   op init32 (f:int -> W32.t) =
-    init (fun i => f (i %/ 4) \bits8 (i%%4)).    
+    init (fun i => f (i %/ 4) \bits8 (i%%4)).
 
   op init64 (f:int -> W64.t) =
-    init (fun i => f (i %/ 8) \bits8 (i%%8)).    
+    init (fun i => f (i %/ 8) \bits8 (i%%8)).
 
-  op init128 (f:int -> W128.t) = 
-    init (fun i => f (i %/ 16) \bits8 (i%%16)).  
+  op init128 (f:int -> W128.t) =
+    init (fun i => f (i %/ 16) \bits8 (i%%16)).
 
-  op init256 (f:int -> W256.t) = 
-    init (fun i => f (i %/ 32) \bits8 (i%%32)).  
+  op init256 (f:int -> W256.t) =
+    init (fun i => f (i %/ 32) \bits8 (i%%32)).
 
 end WArray.
 
@@ -256,7 +256,7 @@ clone export WArray as WArray45  with op size <- 45.
 clone export WArray as WArray46  with op size <- 46.
 clone export WArray as WArray47  with op size <- 47.
 clone export WArray as WArray48  with op size <- 48.
-clone export WArray as WArray49  with op size <- 49. 
+clone export WArray as WArray49  with op size <- 49.
 *)
 
 
